StateSpace/Definitions.v
@@ -1,0 +1,1033 @@
+Require Import Base.
+Require Import Circuit.
+Require Import Monad.
+Require Import Setoid.
+
+Require Import List.
+Import ListNotations.
+Open Scope list_scope.
+
+Import EnsembleNotation.
+Open Scope ensemble_scope.
+
+
+(** * Define a state space for modeling asynchronous controllers, based loosely
+on trace theory *)
+Section state_space.
+
+
+(** In this section we will use Ensembles heavily, and for the sake of
+consistency we will assume there is an abstract type [name] that all the
+Ensembles will quantify over. *)
+Variable name : Set.
+Context `{name_eq_dec : eq_dec name}.
+
+
+(** An event is an element of an ensemble exactly if its underlying key is in the ensemble. *)
+Inductive event_in {val} (I : Ensemble name) : option (event name val) -> Prop :=
+| Event_In i (pf : i ∈ I) v : event_in I (Some (Event i v)).
+
+Lemma not_event_in : forall {val} x (v : val) I, ~ event_in I (Some (Event x v)) -> x ∉ I.
+Proof.
+ intros. intro. apply H. constructor. auto.
+Qed.
+Lemma in_implies_event_in : forall (x : name) X (v : value),
+  x ∈ X ->
+  event_in X (Some (Event x v)).
+Proof.
+  intros. econstructor. auto.
+Qed.
+Lemma not_in_implies_event_not_in : forall (x : name) X (v : value),
+  x ∉ X ->
+  ~ event_in X (Some (Event x v)).
+Proof.
+  intros. inversion 1; subst. contradiction.
+Qed.
+
+Add Parametric Morphism : event_in
+  with signature Same_set name ==> @eq (option (event name value)) ==> iff as event_in_equiv.
+Proof.
+  intros X Y Hequiv e.
+  split; intros Hin; inversion Hin; subst; constructor; rewrite Hequiv in *; auto.
+Qed.
+
+
+(** A state space consists of 
+
+1. a set of input wires
+2. a set of output wires
+3. a set of internal wires (not visible in the events of the transition relation
+4. a transition relation
+
+The transition relation for a state space [C] holds of the triple ([σ],[e],[τ]),
+also written [C ⊢ σ →{e} τ], if the state [σ] transitions to the state [τ] via
+the event [e]. In this case, [e] may be either an actual event ([Some e']) or an
+epsilon transition ([None]), and [τ] may be an actual state ([Some σ']) or the
+error state ([None]).
+
+The transition relation is a relation and not a function primarily because of
+the presence of epsilon transitions.
+
+*)
+Record StateSpace :=
+  { space_input : Ensemble name
+  ; space_output : Ensemble name
+  ; space_internal : Ensemble name
+  ; space_step  : state name -> option (event name value) -> option (state name) -> Prop
+  }.
+
+(** The domain of a state space is the union of its input, output, and internal wires *)
+Definition space_domain (S : StateSpace) := space_input S ∪ space_output S ∪ space_internal S.
+
+Notation "C ⊢ σ →{ e } τ" := (space_step C σ e τ) (no associativity, at level 70).
+
+(** The multi-step relation [C ⊢ σ →*{t} τ] is the closure of the step relation
+over a trace of events. Note that epsilon transitions are not present in the
+trace. *)
+Reserved Notation "C ⊢ σ →*{ t } τ" (no associativity, at level 70).
+Inductive space_steps (C : StateSpace) (σ : state name)
+          : trace name value -> option (state name) -> Prop :=
+| steps0 : C ⊢ σ →*{t_empty} Some σ
+| steps1 σ' t e τ :
+    C ⊢ σ →*{t} Some σ' ->
+    C ⊢ σ' →{Some e} τ ->
+    C ⊢ σ →*{t ▶ e} τ
+| stepsEps σ' t τ :
+    C ⊢ σ →*{t} Some σ' ->
+    C ⊢ σ' →{None} τ ->
+    C ⊢ σ →*{t} τ
+where "C ⊢ σ →*{ t } τ" := (space_steps C σ t τ).
+
+Definition traces_of (S : StateSpace) (σ0 : state name) : Ensemble (trace name value) :=
+  fun t => exists σ, S ⊢ σ0 →*{t} Some σ.
+
+  Definition state_equiv_on (X : Ensemble name) (τ1 τ2 : option (state name)) :=
+      match τ1, τ2 with
+      | Some σ1, Some σ2 => forall x, x ∈ X -> σ1 x = σ2 x
+      | None, None => True
+      | _, _ => False
+      end.
+
+
+  Add Parametric Morphism : state_equiv_on
+    with signature (Same_set name) ==> (@eq (option (state name)))
+                                   ==> (@eq (option (state name))) ==> iff
+    as state_equiv_on_equiv.
+  Proof.
+    intros X Y HXY τ τ'.
+    split; intros Hequiv.
+    * destruct τ as [σ | ]; destruct τ' as [σ' | ]; try inversion Hequiv.
+      { simpl in *.
+        intros x Hx.
+        rewrite <- HXY in Hx.
+        apply Hequiv; auto.
+      }
+      { constructor. }
+    * destruct τ as [σ | ]; destruct τ' as [σ' | ]; try inversion Hequiv.
+      { simpl in *.
+        intros x Hx.
+        rewrite HXY in Hx.
+        apply Hequiv; auto.
+      }
+      { constructor. }
+  Qed.
+
+  Ltac rewrite_state_equiv_on :=
+  match goal with
+  | [ Hequiv : state_equiv_on _ (Some ?σ) _ |- context[?σ _] ] =>
+    rewrite Hequiv; [ | try solve_set; try (decompose_set_structure; solve_set); fail]
+  | [ Hequiv : state_equiv_on _ _ (Some ?σ) |- context[?σ _] ] =>
+    rewrite <- Hequiv; [ | try solve_set; try (decompose_set_structure; solve_set); fail]
+  end.
+
+
+(** A state space is well-formed if several properties hold. There may be other
+properties that also hold not included here, such as the condition that each
+input/output/internal set are individually all_disjoint, or that the transition
+relation is only valid for events in [space_input S ∪ space_outupt S]. *)
+Record well_formed (S : StateSpace) :=
+  { (*space_dom : forall x, x ∈ space_domain S <-> in_fin_state σ x*)
+    space_input_output : space_input S ⊥ space_output S
+  ; space_input_internal : space_input S ⊥ space_internal S
+  ; space_output_internal : space_output S ⊥ space_internal S
+  ; wf_space : forall σ x v τ,
+    S ⊢ σ →{Some (Event x v)} τ ->
+    x ∈ space_input S ∪ space_output S
+  ; wf_scoped : forall σ e σ',
+    S ⊢ σ →{e} Some σ' ->
+    forall x, (forall v, e <> Some (Event x v)) ->
+              x ∈ space_input S ∪ space_output S ->
+              σ' x = σ x
+  ; wf_update : forall σ x v σ',
+    S ⊢ σ →{Some (Event x v)} Some σ' ->
+    σ' x = v
+  }.
+
+
+
+(** A state [σ] in the state space [S] is stable if the only events that are
+enabled in σ are input events. That is, S will not take any more steps except
+those prompted by the environment. *)
+Record stable (S : StateSpace) (σ : state name) :=
+  { stable_wf : well_formed S
+  ; stable_step : forall e τ, S ⊢ σ →{e} τ -> event_in (space_input S) e }.
+
+Class stable_dec (S : StateSpace) :=
+  { space_stable_dec : forall σ, stable S σ + ~ stable S σ }.
+
+
+
+(** * Define a circuit state space from a combinational logic function *)
+Section FuncStateSpace.
+
+  Variable I : list name.
+  Variable x : name.
+  Variable f : state name -> value.
+  Hypothesis x_notin_I : ~ (x ∈ from_list I).
+
+  Let dom := from_list I ∪ singleton x ∪ ∅.
+  Hint Unfold dom.
+  Lemma x_in_dom : x ∈ dom. unfold dom. auto with sets. Qed.
+  Lemma I_subset_dom : forall i, i ∈ from_list I -> i ∈ dom.
+  Proof. unfold dom. auto with sets. Qed.
+
+  (** The definition of func_step requires a notion of stability of the state
+  space, which in this case corresponds to [x] being equal to the value of
+  [f(I)] in [σ]. Below we will prove that this condition exactly correlates with
+  the stability of the state space. *)
+  Let func_stable (σ : state name) := σ x = f σ.
+  Hint Unfold func_stable.
+  
+  Inductive func_step (σ : state name) :
+                      option (event name value) ->
+                      option (state name) ->
+                      Prop :=
+  | func_input_stable i (pf_i : i ∈ from_list I) v σ' :
+    func_stable σ ->
+(*    σ i <> v -> *) (* Question: what happens if an event occurs that doesn't change the value of the variable? Is it allowed? Is it a no-op? *)
+    state_equiv_on (from_list I ∪ singleton x) (Some (update σ i v)) (Some σ') ->
+    func_step σ (Some (Event i v))
+                (Some σ')
+
+  | func_input_unstable i (pf_i : i ∈ from_list I) v σ' :
+    ~ (func_stable σ) ->
+(*    ~ (func_stable (update σ i v)) -> (* in a binary system, this is ok *)*)
+    f σ = f (update σ i v) -> (* ok to update input in an unstable system if the output doesn't change *)
+    state_equiv_on (from_list I ∪ singleton x) (Some (update σ i v))  (Some σ') ->
+    func_step σ (Some (Event i v)) (Some σ')
+
+
+  (* if input updates in an unstable system causes output to change, go to error state*)
+  | func_err i (pf_i : i ∈ from_list I) v :
+    ~ (func_stable σ) ->
+    f σ <> f (update σ i v) -> 
+    func_step σ (Some (Event i v)) None
+
+  | func_output v σ' :
+    ~ (func_stable σ) ->
+    v = f σ ->
+    state_equiv_on (from_list I ∪ singleton x) (Some (update σ x v)) (Some σ')  ->
+    func_step σ (Some (Event x v))
+                (Some σ')
+  .
+
+  Program Definition func_space : StateSpace :=
+  {| space_input := from_list I
+   ; space_output := singleton x
+   ; space_internal := ∅
+   ; space_step := func_step
+   |}.
+
+
+  Lemma func_wf : well_formed func_space.
+  Proof.
+    split.
+    + constructor.
+      simpl.
+      intros y Hy.
+      decompose_set_structure.
+    + constructor.
+      simpl.
+      intros y Hy.
+      decompose_set_structure.
+    + constructor.
+      simpl.
+      intros y Hy.
+      decompose_set_structure.
+    + intros σ y v σ' Hstep.
+      inversion Hstep; try (subst; solve_set).
+      rewrite <- H. simpl. solve_set
+
+    + intros ? ? ? Hstep y y_neq_z y_not_internal.
+    + intros ? ? ? Hstep y y_neq_z y_not_internal.
+
+      inversion Hstep; try subst; unfold update in *.
+      ++ rewrite_state_equiv_on.
+         assert (i <> y).
+         { intro. apply (y_neq_z v). subst; auto. }
+         reduce_eqb; auto.
+      ++ rewrite_state_equiv_on.
+         assert (i <> y).
+         { intro. apply (y_neq_z v). subst; auto. }
+         reduce_eqb; auto.
+      ++ rewrite_state_equiv_on.
+         compare x y; auto.
+         { (* x = y *)
+            rewrite Heq in y_neq_z.
+            specialize (y_neq_z (f σ) eq_refl).
+            find_contradiction.
+         }
+
+    + intros ? y ? ? Hstep.
+      inversion Hstep; try subst; unfold update in *;
+        rewrite_state_equiv_on;
+        reduce_eqb; auto.
+  Qed.
+
+  (** ** Decidability of stability for function spaces *)
+
+  (** This just depends on the enumerability of I *)
+(*  Hypothesis space_wf_decidable : forall σ, well_formed func_space σ + ~(well_formed func_space σ).*)
+
+  Lemma func_stable_equiv : forall σ, 
+        func_stable σ <-> stable func_space σ.
+  Proof.
+    intros σ. split; intros Hstable.
+    * (*destruct Hstable as [H_x_stable H_I_stable].*)
+      split; [apply func_wf | ].
+      intros e τ Hstep.
+      inversion Hstep; subst.
+      + constructor. auto.
+      + contradiction.
+      + contradiction.
+      + contradiction.
+    * compare (σ x) (f σ); auto.
+
+      inversion Hstable.
+      assert (Hstep : func_space ⊢ σ →{Some (Event x (f σ))} Some (update σ x (f σ))).
+      { apply func_output; auto.
+        intros y Hy. unfold update. compare_next; auto. }
+      specialize (stable_step0 _ _ Hstep).
+      inversion stable_step0; subst.
+      simpl in *. find_contradiction.
+  Qed.
+
+
+  Instance func_stable_dec : stable_dec func_space.
+  Proof.
+    split.
+    intros σ.
+    {
+    compare (f σ) (σ x).
+    * left. apply func_stable_equiv; auto.
+
+    * right. intros Hstable. 
+      apply func_stable_equiv in Hstable; auto.
+    }
+  Defined.
+End FuncStateSpace.
+
+
+(** * Composition of two state spaces, written S1 ∥ S2. *)
+Section UnionStateSpace.
+
+  Variable S1 S2 : StateSpace.
+  Hypothesis output_dec1 : in_dec (space_output S1).
+  Hypothesis output_dec2 : in_dec (space_output S2).
+
+  (** The union is only defined for two spaces that are appropriately disjoint. The spaces may share input wires with the others' output wires, however. *)
+
+  Hypothesis output_disjoint : space_output S1 ⊥ space_output S2.
+  Hypothesis wires1_disjoint : space_internal S1 ⊥ space_domain S2.
+  Hypothesis wires2_disjoint : space_domain S1 ⊥ space_internal S2.
+
+  Let union_input := (space_input S1 ∖ space_output S2) ∪ (space_input S2 ∖ space_output S1).
+  Let union_output := space_output S1 ∪ space_output S2.
+  Let union_internal := space_internal S1 ∪ space_internal S2.
+  Hint Unfold union_input union_output union_internal.
+
+  Inductive union_input_event (e : option (event name value)) :=
+  | driven_by_1 : event_in (space_output S1) e ->
+              event_in (space_input S2) e ->
+              union_input_event e
+  | driven_by_2 : event_in (space_input S1) e ->
+              event_in (space_output S2) e ->
+              union_input_event e
+  | driven_by_env : event_in (space_input S1) e ->
+                event_in (space_input S2) e ->
+                union_input_event e.
+
+  Context `{in_dec _ (space_domain S1)} `{in_dec _ (space_domain S2)}.
+
+
+  Inductive union_state : option (state name) -> option (state name) -> option (state name) -> Prop :=
+  | union_None1 τ : union_state None τ None
+  | union_None2 τ : union_state τ None None
+  | union_Some : forall σ1 σ2 σ,
+    (forall y, y ∉ space_internal S2 -> σ y = σ1 y) ->
+    (forall y, y ∉ space_internal S1 -> σ y = σ2 y) ->
+    union_state (Some σ1) (Some σ2) (Some σ)
+  .
+
+  Inductive union_step (σ : state name)
+                     : option (event name value) ->
+                       option (state name) ->
+                       Prop :=
+  | union_step_1 e τ :
+    ~ (event_in (space_domain S2) e) ->
+    S1 ⊢ σ →{e} τ ->
+    state_equiv_on (space_domain S2) (Some σ) τ ->
+    union_step σ e τ
+
+  | union_step_2 e τ :
+    ~ (event_in (space_domain S1) e) ->
+    S2 ⊢ σ →{e} τ ->
+    state_equiv_on (space_domain S1) (Some σ) τ ->
+    union_step σ e τ
+
+  | union_communicate e τ :
+    union_input_event e ->
+    S1 ⊢ σ →{e} τ ->
+    S2 ⊢ σ →{e} τ ->
+    union_step σ e τ
+    .
+
+    
+  Definition union : StateSpace :=
+    {| space_input := union_input
+     ; space_output := union_output
+     ; space_internal := union_internal
+     ; space_step := union_step
+    |}.
+
+
+  Definition union_stable (σ : state name) := 
+    stable S1 σ /\ stable S2 σ.
+
+
+  Lemma wf_union : 
+    well_formed S1 ->
+    well_formed S2 ->
+    well_formed union.
+  Proof.
+  intros [disjoint_in_out1 disjoint_in_int1 disjoint_out_int1 wf1]
+         [disjoint_in_out2 disjoint_in_int2 disjoint_out_int2 wf2].
+  constructor;
+    simpl in *;
+      unfold union_input, union_output, union_internal in *.
+    
+  - constructor; intros x Hintersect; decompose_set_structure.
+  - constructor; intros x Hintersect; decompose_set_structure.
+    { destruct wires1_disjoint as [Hdisjoint].
+      apply (Hdisjoint x). unfold space_domain. solve_set.
+    }
+    { destruct wires2_disjoint as [Hdisjoint].
+      apply (Hdisjoint x). unfold space_domain. solve_set.
+    } 
+  - constructor; intros x Hintersect; decompose_set_structure.
+    { destruct wires1_disjoint as [Hdisjoint].
+      apply (Hdisjoint x). unfold space_domain. solve_set.
+    }
+    { destruct wires2_disjoint as [Hdisjoint].
+      apply (Hdisjoint x). unfold space_domain. solve_set.
+    } 
+  - intros ? ? ? ? Hstep.
+    simpl. unfold union_input, union_output.
+    inversion Hstep; subst.
+    * apply wf1 in H2.
+      simpl. unfold union_input, union_output.
+      decompose_set_structure.
+      { assert (x ∉ space_output S2).
+        { intro. apply H1. constructor; auto. unfold space_domain. solve_set. }
+        solve_set.
+      }
+    * apply wf2 in H2.
+      decompose_set_structure.
+      assert (x ∉ space_output S1).
+      { intro. apply H1. constructor; auto. unfold space_domain. solve_set. }
+      solve_set.
+    * inversion H1.
+      + inversion H4; subst. inversion H5; subst.
+        solve_set.
+      + inversion H4; subst. inversion H5; subst.
+        solve_set.
+      + inversion H4; subst. inversion H5; subst.
+        assert (x ∉ space_output S1).
+        { intro. inversion disjoint_in_out1 as [wf].
+          apply (wf x).
+          solve_set.
+        }
+        solve_set.
+
+  - intros ? ? ? Hstep x Hx x_not_internal.
+    decompose_set_structure;
+      inversion Hstep; subst;
+      try match goal with
+      | [ H : ?x ∈ space_input ?S
+        , Hstep : ?S ⊢ ?σ →{e} Some ?σ'
+        , Hscoped : forall σ e σ', ?S ⊢ σ →{e} Some σ' ->
+                    forall x, (forall v, e <> Some (Event x v)) ->
+                    x ∈ space_input ?S ∪ space_output ?S -> σ' x = σ x
+        |- ?σ' ?x = ?σ ?x ] => apply (Hscoped _ _ _ Hstep); [ auto | solve_set ]; fail
+      | [ H : ?x ∈ space_output ?S
+        , Hstep : ?S ⊢ ?σ →{e} Some ?σ'
+        , Hscoped : forall σ e σ', ?S ⊢ σ →{e} Some σ' ->
+                    forall x, (forall v, e <> Some (Event x v)) ->
+                    x ∈ space_input ?S ∪ space_output ?S -> σ' x = σ x
+        |- ?σ' ?x = ?σ ?x ] => apply (Hscoped _ _ _ Hstep); [ auto | solve_set ]; fail
+
+      | [ H : ?x ∈ space_input ?S
+        , Hstep : state_equiv_on (space_domain ?S) (Some ?σ) (Some ?σ')
+        |- ?σ' x = σ x ] => rewrite Hstep; unfold space_domain; solve_set; fail
+      | [ H : ?x ∈ space_output ?S
+        , Hstep : state_equiv_on (space_domain ?S) (Some ?σ) (Some ?σ')
+        |- ?σ' x = σ x ] => rewrite Hstep; unfold space_domain; solve_set; fail
+
+      end.
+
+  - intros ? ? ? ? Hstep.
+    inversion Hstep; subst.
+    + eapply wf_update0; eauto.
+    + eapply wf_update1; eauto.
+    + erewrite wf_update0; eauto.
+  Qed.
+
+
+  (** Although this direction ([union_stable_implies]) is true, I don't know if the other direction
+  actually is true, e.g. if [S1 ∥ S2] is stable, then both [S1] and [S2] are
+  stable. If it is true, I may have to make some subtle arguments about the fact
+  that certain (e.g. input events) are always enabled in a state. *)
+  Lemma union_stable_implies : forall σ, 
+        stable S1 σ ->
+        stable S2 σ ->
+        stable union σ.
+  Proof.
+    intros σ Hstable1 Hstable2.
+    * split; auto.
+      + destruct Hstable1, Hstable2.
+        apply wf_union; auto.
+      + intros e τ Hstep.
+           destruct Hstable1 as [Hwf1 Hstable1];
+           destruct Hstable2 as [Hwf2 Hstable2].
+        destruct Hstep.
+        ++ assert (He : event_in (space_input S1) e).
+           { eapply Hstable1; eauto. }
+           inversion He; subst.
+           constructor. simpl. unfold union_input.
+           assert (Hi' : ~(i ∈ space_output S2)).
+           { intros He'. apply H1.
+             constructor. simpl. unfold space_domain. auto with sets. }
+           auto with sets.
+        ++ assert (He : event_in (space_input S2) e).
+           { eapply Hstable2; eauto. }
+           inversion He; subst.
+           constructor. simpl. unfold union_input.
+           assert (Hi' : ~(i ∈ space_output S1)).
+           { intros He'. apply H1.
+             constructor. simpl. unfold space_domain. auto with sets. }
+           auto with sets.
+        ++ assert (He1 : event_in (space_input S1) e).
+           { eapply Hstable1; eauto. }
+           assert (He2 : event_in (space_input S2) e).
+           { eapply Hstable2; eauto. }
+           inversion He1; subst.
+           inversion He2; subst.
+           constructor. simpl. unfold union_input.
+           left. constructor; auto.
+           intro.
+           inversion Hwf2 as [[Hwf2']].
+           apply (Hwf2' i).
+           auto with sets.
+  Qed.
+End UnionStateSpace.
+
+
+(** * Move a name from the output of a state space to the input of a state space. *)
+Section HideStateSpace.
+
+  Variable x : name.
+  Variable S : StateSpace.
+
+  Hypothesis x_output : x ∈ space_output S.
+
+  Let hide_input := space_input S.
+  Let hide_output := space_output S ∖ singleton x.
+  Let hide_internal := space_internal S ∪ singleton x.
+
+  Inductive hide_step (σ : state name) :
+                      option (event name value) ->
+                      option (state name) ->
+                      Prop :=
+  | Hide_Eq v τ:
+    S ⊢ σ →{Some (Event x v)} τ ->
+    hide_step σ None τ
+  | Hide_Neq e τ :
+    S ⊢ σ →{e} τ ->
+    ~(event_in (singleton x) e) ->
+    hide_step σ e τ
+  .
+
+  Definition hide : StateSpace :=
+    {| space_input := hide_input
+     ; space_output := hide_output
+     ; space_internal := hide_internal
+     ; space_step := hide_step
+    |}.
+
+
+  Lemma hide_wf : well_formed S -> well_formed hide.
+  Proof.
+    intros [[wfIO] [wfII] [wfOI] wfStep].
+    constructor; simpl; unfold hide_input, hide_output, hide_internal.
+    - constructor. intros y Hy.
+      decompose_set_structure.
+      apply (wfIO y). solve_set.
+    - constructor. intros y Hy.
+      decompose_set_structure.
+      { apply (wfII y). solve_set. }
+      { apply (wfIO x). solve_set. }
+    - constructor. intros y Hy.
+      decompose_set_structure.
+      { apply (wfOI y). solve_set. }
+    - intros σ y v σ' Hstep.
+      inversion Hstep; subst.
+      assert (x <> y).
+      { intro. apply H0. constructor. subst. auto with sets. }
+      specialize (wfStep _ _ _ _ H).
+      decompose_set_structure.
+      solve_set.
+    - intros ? ? ? Hstep y Hy y_not_internal.
+      decompose_set_structure;
+      inversion Hstep; subst;
+      repeat match goal with
+      | [ H : ?x ∈ space_input ?S
+        , Hstep : ?S ⊢ ?σ →{?e} Some ?σ'
+        , Hscoped : forall σ e σ', ?S ⊢ σ →{e} Some σ' ->
+                    forall x, (forall v, e <> Some (Event x v)) ->
+                    x ∈ space_input ?S ∪ space_output ?S -> σ' x = σ x
+        |- ?σ' ?x = ?σ ?x ] => apply (Hscoped _ _ _ Hstep);
+           [ auto; intro; inversion 1; subst; find_contradiction | solve_set ]
+      | [ H : ?x ∈ space_output ?S
+        , Hstep : ?S ⊢ ?σ →{?e} Some ?σ'
+        , Hscoped : forall σ e σ', ?S ⊢ σ →{e} Some σ' ->
+                    forall x, (forall v, e <> Some (Event x v)) ->
+                    x ∈ space_input ?S ∪ space_output ?S -> σ' x = σ x
+        |- ?σ' ?x = ?σ ?x ] => apply (Hscoped _ _ _ Hstep);
+           [ auto; intro; inversion 1; subst; find_contradiction | solve_set ]
+
+      | [ Hinput : ?x ∈ ?A
+        , Houtput : ?x ∈ ?B
+        , Hwf : forall x, x ∉ ?A ∩ ?B |- _ ] => contradiction (Hwf x); solve_set
+
+      end.
+
+
+    - intros ? ? ? ? Hstep.
+      inversion Hstep; subst; auto.
+      eapply wf_update0; eauto.
+  Qed.
+End HideStateSpace.
+
+
+
+(** * A state space modeling a D-flip-flop with set and reset lines. *)
+Section Flop.
+
+  (* the set and reset lines can be optional*)
+  Variable set reset : name.
+  Variable clk old_clk : name.
+  Variable D Q : name.
+
+  Context (disjoint : all_disjoint [set; reset;clk;old_clk;D;Q]).
+  Let flop_input := from_list [set;reset;clk;D].
+  Let flop_output := singleton Q.
+  Let flop_internal := singleton old_clk.
+
+(*
+  Let Q_output σ :=
+    match σ set with
+    | Num 0 => Num 1
+    | Num 1 => match σ reset with
+               | Num 0 => Num 0
+               | Num 1 => σ D
+               | _     => X
+               end
+    | _     => X
+    end.
+*)
+  Let Q_output σ :=
+    if σ set =? Num 0 then Num 1
+    else if σ reset =? Num 0 then Num 0
+    else σ D.
+
+  Let flop_stable σ :=
+    σ Q = Q_output σ /\ σ clk = σ old_clk.
+
+  Inductive flop_step (σ : state name) :
+                      option (event name value) ->
+                      option (state name) ->
+                      Prop :=
+    (* an input is allowed when, either (1) the flip-flop is stable aka any
+    possible clock changes have been registered; or (2) when the input would not
+    actually be observable on the outputs of the circuit. *)
+  | Flop_input i v σ' :
+    flop_stable σ \/ Q_output σ = Q_output (update σ i v) ->
+    i ∈ flop_input ->
+    state_equiv_on (from_list [set;reset;clk;D;Q;old_clk]) (Some (update σ i v)) (Some σ') ->
+    flop_step σ (Some (Event i v)) (Some σ')
+
+    (* other inputs lead to the error state *)
+  | Flop_input_err i v :
+    ~ flop_stable σ ->
+    Q_output σ <> Q_output (update σ i v) ->
+    i ∈ flop_input ->
+    flop_step σ (Some (Event i v)) None
+
+    (* if the set line is high, raise Q *)
+  | Flop_set σ' :
+    σ set = Num 0 ->
+    σ Q  <> Num 1 ->
+    state_equiv_on (from_list [set;reset;clk;D;Q;old_clk]) (Some (update σ Q (Num 1))) (Some σ') ->
+    flop_step σ (Some (Event Q (Num 1))) (Some σ')
+
+    (* if the reset line is high, lower Q *)
+  | Flop_reset σ' :
+    σ set   = Num 1 ->
+    σ reset = Num 0 ->
+    σ Q    <> Num 0 ->
+    state_equiv_on (from_list [set;reset;clk;D;Q;old_clk]) (Some (update σ Q (Num 0))) (Some σ') ->
+    flop_step σ (Some (Event Q (Num 0))) (Some σ')
+
+    (* if the clock has fallen (i.e. input changed and clk is no longer 1), do
+    nothing to the outputs, but propogate thd change to the old_clk. *)
+  | Flop_clk_fall σ' :
+    σ clk <> Num 1 ->
+    σ clk <> σ old_clk ->
+    state_equiv_on (from_list [set;reset;clk;D;Q;old_clk]) (Some (update σ old_clk (σ clk)))
+                                                           (Some σ')
+                                                            ->
+    flop_step σ None (Some σ')
+
+    (* if the clock has risen (i.e. input changed and clk is now equal to 1),
+    update Q and old_clk to their proper values. The result will now be stable *)
+  | Flop_clk_rise v σ' :
+    σ set      = Num 1 ->
+    σ reset    = Num 1 ->
+    σ clk      = Num 1 ->
+    σ old_clk <> Num 1 ->
+
+    v = σ D ->
+    state_equiv_on (from_list [set;reset;clk;D;Q;old_clk])
+                   (Some (update (update σ Q v) old_clk (σ clk)))
+                   (Some σ') ->
+
+    flop_step σ (Some (Event Q v)) (Some σ')
+  .
+
+  Definition flop : StateSpace :=
+    {| space_input := flop_input
+     ; space_output := flop_output
+     ; space_internal := flop_internal
+     ; space_step := flop_step
+    |}.
+
+
+  Lemma flop_wf : well_formed flop.
+  Proof.
+      constructor; simpl in *; unfold flop_input, flop_output, flop_internal in *.
+      + constructor.
+        intros x Hx.
+        decompose_set_structure.
+      + constructor.
+        intros x Hx.
+        decompose_set_structure.
+      + constructor.
+        intros x Hx.
+        decompose_set_structure.
+      + intros ? ? ? ? Hstep.
+        inversion Hstep; try subst; try solve_set.
+      + intros ? ? ? Hstep y Hy H_not_internal.
+        decompose_set_structure;
+        inversion Hstep; try subst;
+        repeat match goal with
+        | [ H : forall v0, Some (Event ?x ?v) <> Some (Event ?x v0)
+          |- _ ] => contradiction (H v); auto
+        | [ H : state_equiv_on _ _ (Some ?σ')
+          |- ?σ' _ = _ ] =>
+          rewrite <- H; [ unfold update; repeat compare_next; auto | solve_set]
+        end.
+    + intros ? ? ? ? Hstep.
+      inversion Hstep; try subst; unfold update; reduce_eqb; auto.
+      ++ unfold flop_input in *. rewrite_state_equiv_on. 
+         unfold update. reduce_eqb; auto.
+      ++ rewrite_state_equiv_on.
+         unfold update.
+         reduce_eqb; auto.
+      ++ rewrite_state_equiv_on.
+         unfold update.
+         reduce_eqb; auto.
+      ++ rewrite_state_equiv_on.
+         unfold update.
+         reduce_eqb; auto.
+         compare_next; auto.
+  Qed.
+
+  Lemma flop_output_is_bit : forall σ v σ',
+    val_is_bit (σ D) ->
+    flop ⊢ σ →{Some (Event Q v)} Some σ' ->
+    val_is_bit v.
+  Proof.
+    intros ? ? ? ? Hstep.
+    inversion Hstep as [? ? ? ? Hi | | | | |]; subst;
+      auto; try constructor.
+    * contradict Hi. unfold flop_input. solve_set.
+  Qed.
+
+
+  Lemma flop_old_clk : forall σ x v σ',
+    val_is_bit v ->
+    flop ⊢ σ →{Some (Event x v)} Some σ' ->
+    val_is_bit (σ clk) ->
+    val_is_bit (σ old_clk) ->
+    val_is_bit (σ' old_clk).
+  Proof.
+    intros ? ? ? ? ? Hstep ? ?.
+    inversion Hstep as [? ? ? ? Hi | | | | |]; try subst; unfold update;
+      try match goal with
+      | [ H : state_equiv_on _ _ (Some ?σ') |- _ ] =>
+        rewrite <- H; [try unfold update; repeat (compare_next; auto) | solve_set]
+      end.
+  Qed.
+    
+
+  Lemma flop_stable_implies_stable : forall σ, 
+    flop_stable σ -> stable flop σ.
+  Proof.
+    intros σ Hstable.
+    constructor.
+    * (* well-formed *)
+      apply flop_wf.
+    * intros e τ Hstep.
+      destruct Hstep;
+        try contradiction;
+        try (constructor; auto; fail).
+      + absurd (σ Q = Num 1); auto.
+        destruct Hstable as [Hstable _].
+        rewrite Hstable; unfold Q_output.
+        rewrite H; auto.
+      + absurd (σ Q = Num 0); auto.
+        destruct Hstable as [Hstable _].
+        rewrite Hstable; unfold Q_output.
+        rewrite H, H0; auto.
+      + absurd (σ clk = σ old_clk); auto.
+        destruct Hstable as [_ Hstable]; auto.
+      + absurd (σ clk = σ old_clk); try congruence.
+        destruct Hstable as [_ Hstable]; auto.
+  Qed.
+
+(** The reverse is not true as is; flop_stable would need to be more precise as to how we handle
+when set and reset lines are X:
+
+  Lemma stable_implies_flop_stable : forall σ,
+    stable flop σ ->
+    flop_stable σ.
+*)
+End Flop.
+
+
+(** * A state space modeling a C element. *)
+
+Section Celem.
+
+  Variable x1 x2 y : name.
+  Let C_input := Couple _ x1 x2.
+  Let C_output := singleton y.
+  
+  Definition C_elem_output σ := 
+    match σ x1, σ x2 with
+    | Num 0, Num 0 => Num 0
+    | Num 1, Num 1 => Num 1
+    | Num 0, Num 1 => σ y
+    | Num 1, Num 0 => σ y
+    | _, _ => X
+    end.
+  Definition C_elem : StateSpace := func_space [x1;x2] y C_elem_output.
+
+End Celem.
+
+(** * A state space modeling a delay until a guard holds over some sensitive input wires *)
+(** Relative timing constraint *)
+Section Delay.
+
+  Variable x y : name.
+  Variable sensitivities : list name.
+  (** The guard should only depend on the variables in the sensitivites set *)
+  Variable guard : state name -> Prop.
+  Variable guardb : state name -> bool.
+  Hypothesis guardb_equiv : forall σ, guard σ <-> guardb σ = true.
+
+  Inductive delay_step (σ : state name) :
+                      option (event name value) ->
+                      option (state name) ->
+                      Prop :=
+  | delay_input_unstable : forall v, σ x <> v -> σ y <> σ x ->
+                                     delay_step σ (Some (Event x v)) None
+  | delay_input_stable : forall v, σ y = σ x -> delay_step σ (Some (Event x v)) (Some (update σ x v))
+  (* output only transitions when the guard is true *)
+  | delay_output σ' : σ y <> σ x ->
+                   guard σ ->
+                   state_equiv_on (from_list sensitivities ∪ from_list [x;y]) (Some σ')
+                                                                    (Some (update σ y (σ x))) ->
+                   delay_step σ (Some (Event y (σ x))) (Some σ')
+  .
+
+  Definition delay : StateSpace :=
+    {| space_input := singleton x ∪ from_list sensitivities
+     ; space_output := singleton y
+     ; space_internal := ∅
+     ; space_step := delay_step
+    |}.
+
+  Lemma delay_wf : well_formed delay.
+  Admitted.
+
+End Delay.
+
+
+Section DelaySpace.
+  Variable S : StateSpace.
+  Variable sensitivities : list name.
+  (** The guard should only depend on the variables in the sensitivites set *)
+  Variable guard : state name -> Prop.
+
+
+  Inductive delay_space_step (σ : state name) :
+                      option (event name value) ->
+                      option (state name) ->
+                      Prop :=
+  (* input steps are always valid *)
+  | delay_space_input : forall x v τ,
+    S ⊢ σ →{Some (Event x v)} τ ->
+    state_equiv_on (from_list sensitivities) (Some σ) τ ->
+    x ∈ space_input S ->
+    delay_space_step σ (Some (Event x v)) τ
+
+  (* epsilon steps are always valid *)
+  | delay_space_internal : forall τ,
+    S ⊢ σ →{None} τ ->
+    state_equiv_on (from_list sensitivities) (Some σ) τ ->
+    delay_space_step σ None τ
+
+  (* output steps can only happen if the guard is true *)
+  | delay_space_output : forall x v τ,
+    guard σ ->
+    S ⊢ σ →{Some (Event x v)} τ ->
+    x ∈ space_output S ->
+    state_equiv_on (from_list sensitivities) (Some σ) τ ->
+    delay_space_step σ (Some (Event x v)) τ
+  .
+
+  Definition delay_space (guardb : state name -> bool) : StateSpace :=
+    {| space_input := space_input S ∪ from_list sensitivities
+     ; space_output := space_output S
+     ; space_internal := space_internal S
+     ; space_step := delay_space_step
+    |}.
+
+  Variable guardb : state name -> bool.
+  Lemma delay_space_wf :
+    well_formed S ->
+    from_list sensitivities ⊥ space_domain S ->
+    well_formed (delay_space guardb).
+  Proof.
+    intros Hwf Hdisjoint.
+    destruct Hwf.
+    unfold space_domain in Hdisjoint.
+    assert (Hdisjoint1 : from_list sensitivities ⊥ space_input S).
+    { destruct Hdisjoint as [Hdisjoint]. constructor. intros x Hx.
+      apply (Hdisjoint x).
+      decompose_set_structure; solve_set.
+    }
+    assert (Hdisjoint2 : from_list sensitivities ⊥ space_output S).
+    { destruct Hdisjoint as [Hdisjoint]. constructor. intros x Hx.
+      apply (Hdisjoint x).
+      decompose_set_structure; solve_set.
+    }
+    assert (Hdisjoint3 : from_list sensitivities ⊥ space_internal S).
+    { destruct Hdisjoint as [Hdisjoint]. constructor. intros x Hx.
+      apply (Hdisjoint x).
+      decompose_set_structure; solve_set.
+    }
+    split.
+    * simpl. solve_set.
+    * simpl. solve_set.
+    * simpl. solve_set.
+    * intros σ x v τ Hstep.
+      simpl.
+      inversion Hstep; subst.
+      + solve_set.
+      + solve_set.
+    * intros ? ? ? Hstep x Hv Hx.
+      simpl in Hx.
+      decompose_set_structure.
+      { (* x ∈ input *) inversion Hstep; subst;
+        eapply wf_scoped0; eauto; solve_set.
+      }
+      { (* x ∈ sens *) inversion Hstep; subst; rewrite_state_equiv_on; auto. }
+      { (* x ∈ input *) inversion Hstep; subst;
+        eapply wf_scoped0; eauto; solve_set.
+      }
+    * intros ? ? ? ? Hstep.
+      inversion Hstep; subst;
+      eapply wf_update0; eauto.
+  Qed.
+
+  Lemma delay_space_inversion : forall σ e τ,
+    space_input S ⊥ space_output S ->
+    delay_space guardb ⊢ σ →{e} τ ->
+    S ⊢ σ →{e} τ
+    /\ state_equiv_on (from_list sensitivities) (Some σ) τ
+    /\ (event_in (space_output S) e -> guard σ).
+  Proof.
+    intros σ e τ [Hwf] Hstep.
+    inversion Hstep; subst; auto; repeat split; auto.
+    * intros Hin. contradict Hin. inversion 1; subst.
+      contradiction (Hwf x).
+      solve_set.
+    * intros Hin. inversion Hin.
+  Qed.
+End DelaySpace.
+
+
+End state_space.
+
+Arguments event_in {name val}.
+Arguments Event_In {name val}.
+Arguments space_input {name}.
+Arguments space_output {name}.
+Arguments space_internal {name}.
+Arguments space_domain {name}.
+Arguments stable {name}.
+Definition Eps {latch val} : option (event latch val) := None.
+Arguments func_space {name name_eq_dec}.
+Arguments C_elem {name name_eq_dec}.
+Arguments hide {name}.
+Arguments flop {name name_eq_dec}.
+Arguments delay {name name_eq_dec}.
+Arguments delay_space {name}.
+Arguments state_equiv_on {name}.
+Arguments traces_of {name}.
+
+Arguments well_formed {name}.
+Arguments space_input_output {name}.
+Arguments space_input_internal {name}.
+Arguments space_output_internal {name}.
+Arguments wf_space {name}.
+Arguments wf_scoped {name}.
+Arguments wf_update {name}.
+
+Arguments union_input_event {name}.
+
+Notation "C ⊢ σ →{ e } τ" := (space_step _ C σ e τ) (no associativity, at level 70).
+Notation "C ⊢ σ →*{ t } τ" := (space_steps _ C σ t τ) (no associativity, at level 70).
+Notation "S1 ∥ S2" := (union _ S1 S2) (left associativity, at level 91).
