StateSpace/Functional.v
@@ -1,0 +1,1041 @@
+
+Require Import Base.
+Require Import Circuit.
+Require Import Monad.
+Require Import Setoid.
+Require Import StateSpace.Definitions.
+Require Import StateSpace.Tactics.
+Require Import StateSpace.Reflection.
+
+Require Import List.
+Import ListNotations.
+Open Scope list_scope.
+
+Import EnsembleNotation.
+Open Scope ensemble_scope.
+
+Require Import Coq.Logic.FunctionalExtensionality.
+
+Module FunctionalStateSpaces(Export name : NameType).
+  Module Tactics := StateSpaceTactics(name).
+  Export Tactics.
+
+Class functional_step_relation (S : StateSpace name) :=
+  { fun_step : state name -> option (event name value) -> Ensemble (option (state name))
+  ; input_list : enumerable (space_input S)
+  ; output_list : enumerable (space_output S)
+  ; internal_list : enumerable (space_internal S)
+  }.
+Arguments fun_step S {functional_step_relation}.
+Class functional_step_relation_correct (S : StateSpace name) `{functional_step_relation S} :=
+  { fun_step_in : forall σ e τ,
+    S ⊢ σ →{e} τ -> τ ∈ fun_step S σ e
+  ; fun_in_step : forall σ e τ,
+    τ ∈ fun_step S σ e -> S ⊢ σ →{e} τ
+  }.
+Arguments fun_step S {rel} : rename.
+Arguments input_list S {rel} : rename.
+Arguments output_list S {rel} : rename.
+Arguments internal_list S {rel} : rename.
+
+
+Instance functional_step_relation_enumerable_domain S `{H : functional_step_relation S}
+    : enumerable (space_domain S).
+Proof.
+    destruct H. unfold space_domain. typeclasses eauto.
+Defined.
+
+(** Utilities *)
+
+  Fixpoint equiv_on_list' (l : list name) (σ : state name) : Ensemble (state name) :=
+    match l with
+    | nil => fun σ' => True
+    | x :: l' => fun σ' => if σ' x =? σ x
+                           then equiv_on_list' l' σ σ'
+                           else False
+    end.
+  Definition equiv_on_list l σ (τ : option (state name)) : Prop :=
+             match τ with
+             | None => False
+             | Some σ' => equiv_on_list' l σ σ'
+             end.
+
+  Lemma state_equiv_on_implies_list : forall (A : list name) σ τ,
+    state_equiv_on (from_list A) (Some σ) τ ->
+    τ ∈ equiv_on_list A σ.
+  Proof.
+    induction A as [ | a A];
+      intros σ τ Hequiv.
+    * simpl in Hequiv.
+      destruct τ; find_contradiction.
+      constructor.
+    * simpl in Hequiv.
+      unfold equiv_on_list, equiv_on_list'. fold equiv_on_list'.
+      unfold Coq.Sets.Ensembles.In.
+      destruct τ as [ σ' | ]; find_contradiction.
+      rewrite Hequiv; [ | solve_set].
+      reduce_eqb.
+      assert (IH : Some σ' ∈ equiv_on_list A σ).
+      { apply IHA.
+        unfold state_equiv_on.
+        intros y Hy.
+        apply Hequiv. solve_set.
+      }
+      apply IH.
+  Qed.
+
+  Lemma equiv_on_list_implies_state_equiv_on : forall (A : list name) σ τ,
+    τ ∈ equiv_on_list A σ ->
+    state_equiv_on (from_list A) (Some σ) τ.
+  Proof.
+    induction A; intros σ τ Hequiv;
+      unfold Coq.Sets.Ensembles.In in Hequiv.
+    * destruct τ as [σ' | ].
+      2:{ inversion Hequiv. }
+      { simpl. intros y Hx. find_contradiction. }
+    * destruct τ as [σ' | ]; [ | inversion Hequiv].
+      simpl in Hequiv.
+      intros y Hx. simpl in Hx.
+      compare_next.
+      decompose_set_structure.
+      specialize (IHA σ (Some σ')).
+      unfold state_equiv_on in IHA.
+      apply IHA; auto.
+  Qed.
+
+
+  Lemma equiv_on_list_equiv : forall l1 l2 σ,
+    from_list l1 == from_list l2 ->
+    equiv_on_list l1 σ == equiv_on_list l2 σ.
+  (* proving this is trickier than I thought *)
+  Admitted.
+  Lemma in_list_dec_equiv : forall l1 l2 x,
+    from_list l1 == from_list l2 ->
+    in_list_dec x l1 = in_list_dec x l2.
+  Admitted.
+
+
+Ltac deduce_in_domain S :=
+  match goal with
+  | [ Hstep : S ⊢ _ →{ Some (Event ?x _)} _ |- _ ] =>
+    assert (x ∈ space_domain S)
+      by (unfold space_domain;
+          apply wf_space in Hstep; auto;
+          solve_set)
+  | [ He : ~ event_in (space_domain S) (Some (Event ?x _)) |- _ ] =>
+    assert (x ∉ space_domain S)
+      by (intro; apply He; constructor; assumption)
+  | [ He : event_in (space_domain S) (Some (Event ?x _)) |- _ ] =>
+    assert (x ∈ space_domain S)
+      by (inversion He; auto)
+  end.
+
+  Ltac decompose_state_equiv_on :=
+  match goal with
+  | [ H : ?τ ∈ state_equiv_on _ (Some _) |- _ ] =>
+    let σ' := fresh "σ'" in
+    destruct τ as [σ' | ];
+    [ | inversion H; fail]
+  | [ H : ?τ ∈ state_equiv_on _ None |- _ ] =>
+    let σ' := fresh "σ'" in
+    destruct τ as [σ' | ];
+    [ inversion H; fail | ]
+  | [ H : ?τ ∈ singleton None |- _ ] => inversion H
+
+  | [ H :  state_equiv_on _ (Some _) ?τ |- _ ] =>
+    let σ' := fresh "σ'" in
+    destruct τ as [σ' | ];
+    [ | inversion H; fail]
+  | [ H : state_equiv_on _ None ?τ |- _ ] =>
+    let σ' := fresh "σ'" in
+    destruct τ as [σ' | ];
+    [ inversion H; fail | ]
+
+  end.
+
+  Definition event_in_b (X : Ensemble name) `{in_dec _ X} (e : option (event name value)) :=
+    match e with
+    | None => false
+    | Some (Event x v) => if x ∈? X then true else false
+    end.
+
+
+  Section FuncSpace.
+
+  Variable I : list name.
+  Variable x : name.
+  Variable f : state name -> value.
+  Hypothesis x_notin_I : ~ (x ∈ from_list I).
+
+
+  Definition func_step_fun (σ : state name) (e : option (event name value))
+    : Ensemble (option (state name)) :=
+    match e with
+    | None => (* No eps transitions *) ∅
+    | Some (Event z v) =>
+      if in_list_dec z I
+      then if σ x =? f σ
+           then (* func_input_stable *) equiv_on_list (x::I) (update σ z v)
+           else if f σ =? f (update σ z v)
+           then (* func_input_unstable *) equiv_on_list (x::I) (update σ z v)
+           else (* func_err *) singleton None
+      else if z =? x
+      then if σ x =? f σ
+           then (* output cannot transition on stable input *) ∅
+           else if v =? f σ
+           then (* func_output *) equiv_on_list (x::I) (update σ z v)
+           else (* v does not have the correct form *) ∅
+      else (* event ∉ domain(func_space) *) ∅
+      
+    end.
+
+  Lemma func_step_in : forall σ e τ,
+    func_space I x f ⊢ σ →{e} τ ->
+    τ ∈ func_step_fun σ e.
+  Proof.
+    intros σ e τ Hstep.
+    unfold func_step_fun.
+    assert (Heq : from_list I ∪ singleton x == from_list (x::I)).
+    { simpl. split; intros y Hy; decompose_set_structure; solve_set. }
+
+    inversion Hstep; subst.
+    * rewrite_in_list_dec.
+      compare_next; auto.
+      apply state_equiv_on_implies_list.
+      rewrite <- Heq; auto.
+    * rewrite_in_list_dec.
+      compare_next; auto.
+      apply state_equiv_on_implies_list.
+      rewrite <- Heq; auto.
+    * rewrite_in_list_dec.
+      compare_next; auto.
+      solve_set.
+    * destruct (x ∈? from_list I) as [pf_i | pf_i ].
+      { find_contradiction. }
+      { rewrite_in_list_dec. reduce_eqb. 
+        apply state_equiv_on_implies_list.
+        rewrite <- Heq; auto.
+      }
+  Qed.
+
+
+  Lemma func_in_step : forall σ e τ,
+    τ ∈ func_step_fun σ e ->
+    func_space I x f ⊢ σ →{e} τ.
+  Proof.
+    intros σ e τ Hin.
+    unfold func_step_fun in Hin.
+    assert (HxI : from_list I ∪ singleton x == from_list (x::I)).
+    { simpl. split; intros y Hy; decompose_set_structure; solve_set. }
+    destruct e as [[y v] | ]; [ | find_contradiction].
+    destruct (y ∈? from_list I) as [Hy | Hy].
+    { rewrite_in_list_dec.
+      compare_next.
+      { apply equiv_on_list_implies_state_equiv_on in Hin.
+        decompose_state_equiv_on.
+        apply func_input_stable; auto.
+        rewrite HxI; auto.
+      }
+      compare_next.
+      { apply equiv_on_list_implies_state_equiv_on in Hin.
+        decompose_state_equiv_on.
+        apply func_input_unstable; auto.
+        rewrite HxI; auto.
+      }
+      { decompose_state_equiv_on. 
+        apply func_err; auto.
+      }
+    }
+    { rewrite_in_list_dec.
+      compare_next.
+      compare_next.
+      compare_next.
+      apply equiv_on_list_implies_state_equiv_on in Hin.
+      decompose_state_equiv_on.
+      apply func_output; auto.
+      rewrite HxI; auto.
+    }
+  Qed.
+
+
+  Program Instance func_functional : functional_step_relation (func_space I x f) :=
+    {| fun_step := func_step_fun |}.
+  Instance func_functional_correct : functional_step_relation_correct (func_space I x f) :=
+  {| fun_step_in := func_step_in
+   ; fun_in_step := func_in_step
+   |}.
+
+  End FuncSpace.
+
+  Section UnionStateSpace.
+
+  Variable S1 S2 : StateSpace name.
+  Hypothesis output_dec1 : in_dec (space_output S1).
+  Hypothesis output_dec2 : in_dec (space_output S2).
+
+  (** The union is only defined for two spaces that are appropriately disjoint. The spaces may share input wires with the others' output wires, however. *)
+
+  Hypothesis output_disjoint : space_output S1 ⊥ space_output S2.
+  Hypothesis wires1_disjoint : space_internal S1 ⊥ space_domain S2.
+  Hypothesis wires2_disjoint : space_domain S1 ⊥ space_internal S2.
+
+  Context `{S1_functional : functional_step_relation S1}
+          `{S2_functional : functional_step_relation S2}
+          `{S_enumerable : enumerable _ (space_domain S1 ∩ space_domain S2)}.
+  Context `{S1_wf : well_formed S1} `{S2_wf : well_formed S2}.
+
+
+  Fixpoint states_equiv_on (l : list name) (σ1 σ2 : state name) : bool :=
+    match l with
+    | nil => true
+    | x  :: l' => if σ1 x =? σ2 x then states_equiv_on l' σ1 σ2
+                  else false
+    end.
+  Arguments enumerate {A} X.
+
+  Definition join_option_state (τ1 τ2 : option (option (state name))) : option (option (state name)) :=
+    match τ1, τ2 with
+    | None, _ => None
+    | _, None => None
+    | Some None, _ => Some None
+    | _, Some None => Some None
+    | Some (Some σ1), Some (Some σ2) =>
+      if states_equiv_on (enumerate (space_domain S1 ∩ space_domain S2) S_enumerable) σ1 σ2
+      then Some (Some (fun x => if x ∈? space_domain S1
+                                then σ1 x
+                                else σ2 x))
+      else None (* failure if not consistent across states *)
+    end.
+
+
+  Definition union_step_fun (σ : state name) (e : option (event name value))
+        : Ensemble (option (state name)) :=
+    match e with
+    | None =>
+       (fun_step S1 σ None ∩ equiv_on_list (enumerate (space_domain S2) _) σ)
+    ∪ (fun_step S2 σ None ∩ equiv_on_list (enumerate (space_domain S1) _) σ) 
+    | Some (Event x v) =>
+      (* NOTE: we can make assumptions about the well-formedness of S1 ∪ S2
+         because we have assumed these facts. *)
+      if andb (in_list_dec x (enumerate (space_domain S1) _))
+              (in_list_dec x (enumerate (space_domain S2) _))
+      then fun_step S1 σ e ∩ fun_step S2 σ e
+      else if in_list_dec x (enumerate (space_domain S1) _)
+      then (fun_step S1 σ e) ∩ (equiv_on_list (enumerate (space_domain S2) _) σ)
+      else if in_list_dec x (enumerate (space_domain S2) _)
+      then (fun_step S2 σ e) ∩ (equiv_on_list (enumerate (space_domain S1) _) σ)
+      else (* singleton None *) ∅
+    end.
+
+  Instance union_functional : functional_step_relation (S1 ∥ S2) :=
+  {| fun_step := union_step_fun |}.
+  { set (enum_in_1 := input_list S1).
+    set (enum_in_2 := input_list S2).
+    set (enum_out_1 := output_list S1).
+    set (enum_out_2 := output_list S2).
+    typeclasses eauto.
+  }
+  { set (enum_out_1 := output_list S1).
+    set (enum_out_2 := output_list S2).
+    typeclasses eauto.
+  }
+  { set (enum_int_1 := internal_list S1).
+    set (enum_int_2 := internal_list S2).
+    typeclasses eauto.
+  }
+  Defined.
+
+  Context `{S1_functional_correct : @functional_step_relation_correct S1 S1_functional}
+          `{S2_functional_correct : @functional_step_relation_correct S2 S2_functional}.
+
+
+
+  Lemma union_implies_union_step_fun : forall σ e τ,
+    (S1 ∥ S2) ⊢ σ →{e} τ -> τ ∈ union_step_fun σ e.
+  Proof.
+    intros σ e τ Hstep.
+    inversion Hstep; subst;
+      repeat match goal with
+      | [ H : S1 ⊢ _ →{_} _ |- _ ] => rename H into Hstep1
+      | [ H : S2 ⊢ _ →{_} _ |- _ ] => rename H into Hstep2
+      end;
+      try match goal with
+      | [ H : state_equiv_on (space_domain _) (Some _) ?τ |- _ ] =>
+        let σ' := fresh "σ'" in
+        destruct τ as [ σ' | ]; [ | find_contradiction]
+      end.
+
+    * unfold union_step_fun.
+
+      destruct e as [[x v] | ].
+      2:{ left.
+          constructor.
+          { apply (@fun_step_in _ S1_functional); auto. }
+          { apply state_equiv_on_implies_list.
+            rewrite <- rewrite_enumerate; auto.
+          }
+      }
+      { assert (x ∈ space_domain S1).
+        { unfold space_domain.
+          apply wf_space in Hstep1; auto.
+          solve_set.
+        }
+        rewrite_in_list_dec; simpl.
+        assert (x ∉ space_domain S2).
+        { intro. contradict H. constructor; auto. }
+        rewrite_in_list_dec; simpl.
+        split.
+        { apply fun_step_in; auto. }
+        { apply state_equiv_on_implies_list.
+          rewrite <- rewrite_enumerate; auto.
+        }
+      }
+
+
+    * unfold union_step_fun.
+      destruct e as [[x v] | ].
+      2:{ right.
+          split.
+          { apply fun_step_in; auto. }
+          { apply state_equiv_on_implies_list.
+            rewrite <- rewrite_enumerate; auto.
+          }
+      }
+      deduce_in_domain S1; rewrite_in_list_dec.
+      deduce_in_domain S2; rewrite_in_list_dec.
+      simpl.
+
+      split.
+      { apply fun_step_in; auto. }
+      { apply state_equiv_on_implies_list.
+        rewrite <- rewrite_enumerate; auto.
+      }
+
+    * (*rename H3 into Hstep2.*)
+
+      destruct e as [[x v] | ]; simpl.
+      2:{ (* contradiction *)
+          repeat match goal with
+          | [ H : union_input_event _ _ None |- _ ] => inversion H; clear H
+          | [ H : event_in _ None |- _ ] => inversion H; fail
+          end.
+      }
+      deduce_in_domain S1; rewrite_in_list_dec.
+      deduce_in_domain S2; rewrite_in_list_dec.
+      simpl.
+      split; apply fun_step_in; auto.
+  Qed.
+
+  Lemma in_join_domain_implies_union_input_event : forall x v,
+    x ∈ space_domain S1 ->
+    x ∈ space_domain S2 ->
+    union_input_event S1 S2 (Some (Event x v)).
+  Proof.
+    intros x v Hx1 Hx2.
+    unfold space_domain in Hx1, Hx2.
+    destruct (x ∈? from_list (enumerate (space_output S1) (output_list S1)))
+      as  [Houtput1 | Houtput1];
+    rewrite <- rewrite_enumerate in Houtput1.
+    { (* x ∈ output S1 *)
+      (* it must also be the case that x ∈ input S2 *)
+      apply driven_by_1; constructor; auto.
+      decompose_set_structure.
+    }
+    assert (Hx1' : x ∈ space_input S1).
+    { decompose_set_structure; auto.
+      { contradict wires1_disjoint.
+        intros [Hdisjoint].
+        apply (Hdisjoint x).
+        unfold space_domain.
+        solve_set.
+      }
+      { contradict wires1_disjoint.
+        intros [Hdisjoint].
+        apply (Hdisjoint x).
+        unfold space_domain.
+        solve_set.
+      }
+    }
+    destruct (x ∈? from_list (enumerate (space_output S2) (output_list S2)))
+      as  [Houtput2 | Houtput2];
+    rewrite <- rewrite_enumerate in Houtput2.
+    { (* x ∈ output S2 *)
+      (* it must also be the case that x ∈ input S1 *)
+      apply driven_by_2; constructor; auto.
+    }
+    assert (Hx2' : x ∈ space_input S2).
+    { decompose_set_structure; auto. }
+
+    apply driven_by_env; constructor; auto.
+  Qed.
+
+  Lemma union_step_fun_implies_union : forall σ e τ,
+    τ ∈ union_step_fun σ e ->
+    (S1 ∥ S2) ⊢ σ →{e} τ.
+  Proof.
+    intros σ e τ Hstep.
+    unfold union_step_fun in Hstep.
+    destruct e as [[x v] | ].
+    2:{ decompose_set_structure.
+        + apply union_step_1.
+          { inversion 1. }
+          { apply fun_in_step; auto. }
+          { rewrite rewrite_enumerate.
+            apply equiv_on_list_implies_state_equiv_on; auto.
+          }
+            
+        + apply union_step_2.
+          { inversion 1. }
+          { apply fun_in_step; auto. }
+          { rewrite rewrite_enumerate.
+            apply equiv_on_list_implies_state_equiv_on; auto.
+          }
+
+    }
+    { destruct (x ∈? space_domain S1) as [Hx1 | Hx1]; rewrite_in_list_dec; simpl in Hstep;
+      destruct (x ∈? space_domain S2) as [Hx2 | Hx2]; rewrite_in_list_dec; simpl in Hstep.
+      + decompose_set_structure.
+        apply union_communicate; try (apply fun_in_step; auto; fail).
+        { apply in_join_domain_implies_union_input_event; auto. }
+
+      + decompose_set_structure.
+        apply union_step_1.
+        { inversion 1; subst. find_contradiction. }
+        { apply fun_in_step; auto. }
+        { rewrite rewrite_enumerate.
+          apply equiv_on_list_implies_state_equiv_on; auto.
+        }
+      + decompose_set_structure.
+        apply union_step_2.
+        { inversion 1; subst. find_contradiction. }
+        { apply fun_in_step; auto. }
+        { rewrite rewrite_enumerate.
+          apply equiv_on_list_implies_state_equiv_on; auto.
+        }
+      + find_contradiction.
+  }
+  Qed.
+
+(*
+  Lemma dec_union_input_event3 : forall 
+    ~ event_in (space_domain S2) e ->
+    dec_union_input_event e = inright pf.
+  Admitted.
+  Lemma union_step_fun_implies_union : forall σ e τ,
+    union_step_fun σ e = Some τ ->
+    union ⊢ σ →{e} τ.
+  Admitted.
+*)
+  Existing Instance union_functional.
+  Instance union_functional_correct : functional_step_relation_correct (S1 ∥ S2).
+  Proof.
+    split.
+    * apply union_implies_union_step_fun.
+    * apply union_step_fun_implies_union.
+  Qed.
+
+
+End UnionStateSpace.
+
+Section HideStateSpace.
+
+  Variable x : name.
+  Variable S : StateSpace name.
+
+  Hypothesis x_output : x ∈ space_output S.
+
+  Context `{S_functional : functional_step_relation S}.
+  Context `{S_functional_correct : @functional_step_relation_correct S S_functional}.
+  Definition hide_step_fun (σ : state name) (e : option (event name value)) :=
+    match e with
+    | None => (* either an epsilong transition from S, or an x transition from S *)
+      (fun_step S σ None) ∪ (fun τ => exists v, fun_step S σ (Some (Event x v)) τ)
+    | Some (Event y v) =>
+      if x =? y
+      then ∅
+      else fun_step S σ (Some (Event y v))
+    end.
+
+  Lemma hide_fun_step_in : forall σ e τ,
+    hide x S ⊢ σ →{e} τ ->
+    τ ∈ hide_step_fun σ e.
+  Proof.
+    intros σ e τ Hstep.
+    destruct Hstep as [v τ Hstep | e τ Hstep He].
+    * right. exists v.
+      apply fun_step_in; auto.
+    * destruct e as [[y v] | ].
+      + simpl. compare_next.
+        { contradict He. constructor. solve_set. }
+        apply fun_step_in; auto.
+      + left. apply fun_step_in; auto.
+  Qed.
+
+  Lemma hide_fun_in_step : forall σ e τ,
+    τ ∈ hide_step_fun σ e ->
+    hide x S ⊢ σ →{e} τ.
+  Proof.
+    intros σ e τ Hτ. unfold hide_step_fun in Hτ.
+    destruct e as [[y v] | ].
+    * compare_next.
+      { apply Hide_Neq.
+        { apply fun_in_step; auto. }
+        { inversion 1; subst.
+          decompose_set_structure. }
+      }
+    * decompose_set_structure.
+      { apply Hide_Neq.
+        { apply fun_in_step; auto. }
+        { inversion 1. }
+      }
+      { destruct H as [v Hτ].
+        eapply Hide_Eq.
+        apply fun_in_step; eauto.
+      }
+  Qed.
+
+
+  Instance hide_functional : functional_step_relation (hide x S) :=
+  {| fun_step := hide_step_fun |}.
+    * simpl. apply input_list; auto.
+    * simpl.
+      set (Houtput := output_list S).
+      typeclasses eauto.
+    * simpl.
+      set (Houtput := internal_list S).
+      typeclasses eauto.
+  Defined.
+  Instance hide_functional_correct : functional_step_relation_correct (hide x S) :=
+   {| fun_step_in := hide_fun_step_in
+   ; fun_in_step := hide_fun_in_step
+   |}.
+
+End HideStateSpace.
+
+Section Flop.
+
+  (* the set and reset lines can be optional*)
+  Variable set reset : name.
+  Variable clk old_clk : name.
+  Variable D Q : name.
+
+  Context (disjoint : all_disjoint [set; reset;clk;old_clk;D;Q]).
+  Let flop_input := from_list [set;reset;clk;D].
+  Let flop_output := singleton Q.
+  Let flop_internal := singleton old_clk.
+
+  Let Q_output σ :=
+    if σ set =? Num 0 then Num 1
+    else if σ reset =? Num 0 then Num 0
+    else σ D.
+
+  Let update_on_flop σ x v := state_equiv_on (from_list [set;reset;clk;D;Q;old_clk]) (Some (update σ x v)).
+
+  Definition flop_step_fun (σ : state name) (e : option (event name value)) :=
+    match e with
+    | None => (* must be flop_clk_fall *)
+      if σ clk =? Num 1
+      then ∅
+      else if σ clk =? σ old_clk
+      then ∅
+      else update_on_flop σ old_clk (σ clk)
+    | Some (Event x v) =>
+
+      if x ∈? flop_input
+      (* Flop_input *)
+      then if (* flop_stable *) ((σ Q =? Q_output σ) && (σ clk =? σ old_clk))%bool
+           then update_on_flop σ x v
+           else if (* still safe *) Q_output σ =? Q_output (update σ x v)
+           then update_on_flop σ x v
+           else singleton None
+      else if x =? Q
+      then if ((σ set =? Num 0) (* Flop_set *)
+            && negb (σ Q =? Num 1)
+            && (v =? Num 1))%bool
+           then update_on_flop σ Q (Num 1)
+           else if ((σ set =? Num 1) (* Flop_set *)
+                 && (σ reset =? Num 0) (* Flop_reset *)
+                 && negb (σ Q =? Num 0)
+                 && (v =? Num 0))%bool
+                then update_on_flop σ Q (Num 0)
+           else if ((σ set =? Num 1) (* Flop_set *)
+                 && (σ reset =? Num 1) (* Flop_reset *)
+                 && (σ clk =? Num 1) (* Flop_clk_rise *)
+                 && negb (σ old_clk =? Num 1)
+                 && (v =? σ D))%bool
+           then update_on_flop (update σ Q v) old_clk (Num 1)
+           else ∅
+       else ∅
+   end.
+
+
+  Lemma flop_fun_step_in : forall σ e τ,
+    flop set reset clk old_clk D Q ⊢ σ →{e} τ ->
+    τ ∈ flop_step_fun σ e.
+  Proof.
+    intros σ e τ Hstep.
+    destruct Hstep.
+    * unfold flop_step_fun; subst.
+      destruct (i ∈? flop_input); [ | find_contradiction].
+      destruct H as [Hstable | Hchange].
+      + destruct Hstable.
+        compare_next. simpl.
+        unfold update_on_flop.
+        auto.
+      + unfold update_on_flop. 
+        repeat (compare_next; simpl; auto).
+
+    * unfold flop_step_fun.
+      destruct (i ∈? flop_input); [ | find_contradiction].
+      unfold update_on_flop, update, Q_output in *.
+      do 2 (compare_next; simpl; auto; try solve_set).
+      contradict H.
+        compare_next; simpl; auto; try solve_set.
+
+    * unfold flop_step_fun.
+      destruct (Q ∈? flop_input) as [HQ | HQ];
+        [ unfold flop_input in HQ; decompose_set_structure | ].
+      repeat (compare_next; simpl; try solve_set).
+    * subst.  unfold flop_step_fun.
+      destruct (Q ∈? flop_input) as [HQ | HQ];
+        [ unfold flop_input in HQ; decompose_set_structure | ].
+      repeat (compare_next; simpl; try solve_set).
+    * subst.  unfold flop_step_fun.
+      destruct (Q ∈? flop_input) as [HQ | HQ];
+        [ unfold flop_input in HQ; decompose_set_structure | ].
+      repeat (compare_next; simpl; try solve_set).
+    * subst.  unfold flop_step_fun.
+      destruct (Q ∈? flop_input) as [HQ | HQ];
+        [ unfold flop_input in HQ; decompose_set_structure | ].
+      repeat (compare_next; simpl; try solve_set).
+      unfold update_on_flop.
+      repeat my_subst; auto.
+  Qed.
+
+
+
+  Lemma flop_fun_in_step : forall σ e τ,
+    τ ∈ flop_step_fun σ e ->
+    flop set reset clk old_clk D Q ⊢ σ →{e} τ.
+  Proof.
+    intros σ e τ Hstep.
+    unfold flop_step_fun in Hstep.
+    destruct e as [[x v] | ].
+    2:{ compare_next.
+        compare_next.
+        destruct τ as [σ' | ]; [ | inversion Hstep].
+        apply Flop_clk_fall; auto.
+    }
+    unfold update_on_flop in *.
+    destruct (x ∈? flop_input); unfold flop_input in *;
+    repeat (compare_next;
+         simpl in Hstep;
+         try decompose_state_equiv_on;
+         try match goal with
+         | [ |- _ ⊢ _ →{_} Some _ ] =>
+           apply Flop_input; auto; fail
+         | [ |- _ ⊢ _ →{_} None ] =>
+           apply Flop_input_err; auto; try (inversion 1; find_contradiction); fail
+         | [ Heq : ?σ set = Num 0 |- _ ] => apply Flop_set; auto; fail
+         | [ Heq : ?σ reset = Num 0 |- _ ] => apply Flop_reset; auto; fail
+         | [ |- _ ⊢ _ →{ Some (Event Q _) } Some _ ] => apply Flop_clk_rise; auto
+         end).
+    { my_subst. auto. }
+  Qed.
+
+  
+  Instance flop_functional : functional_step_relation (flop set reset clk old_clk D Q) :=
+  {| fun_step := flop_step_fun |}.
+  Instance flop_functional_correct : functional_step_relation_correct (flop set reset clk old_clk D Q ) :=
+  {| fun_step_in := flop_fun_step_in
+   ; fun_in_step := flop_fun_in_step
+   |}.
+
+
+End Flop.
+
+Section DelaySpace.
+
+
+  Variable S : StateSpace name.
+  Variable sensitivities : list name.
+  (** The guard should only depend on the variables in the sensitivites set *)
+  Variable guard : state name -> Prop.
+  Variable guardb : state name -> bool.
+  Hypothesis guardb_equiv : forall σ, guard σ <-> guardb σ = true.
+
+  Context `{S_functional : functional_step_relation S}.
+
+
+  Existing Instance input_list.
+  Existing Instance output_list.
+  Existing Instance internal_list.
+
+
+  Definition delay_space_step_fun σ e : Ensemble (option (state name)) :=
+    match e with
+    | None => (* must come from epsilon step inside S *)
+      fun_step S σ e ∩ equiv_on_list sensitivities σ
+    | Some (Event x v) =>
+      if in_list_dec x (enumerate (space_input S))
+      then fun_step S σ e ∩ equiv_on_list sensitivities σ
+      else if andb (in_list_dec x (enumerate (space_output S)))
+                   (guardb σ)
+      then fun_step S σ e ∩ equiv_on_list sensitivities σ
+      else ∅
+    end.
+
+  Instance delay_space_functional : functional_step_relation (delay_space S sensitivities guard guardb) :=
+  {| fun_step := delay_space_step_fun |}.
+  * simpl. typeclasses eauto.
+  * simpl. typeclasses eauto.
+  Defined.
+
+  Context `{S_functional_correct : @functional_step_relation_correct S S_functional}.
+  
+  Instance delay_space_functional_correct :
+    functional_step_relation_correct (delay_space S sensitivities guard guardb).
+  split.
+  * intros σ e τ Hstep.
+    inversion Hstep; subst; simpl.
+    + rewrite_in_list_dec.
+      split.
+      { eapply fun_step_in; auto. }
+      { apply state_equiv_on_implies_list; auto. }
+    + split.
+      { eapply fun_step_in; auto. }
+      { apply state_equiv_on_implies_list; auto. }
+    + rewrite_in_list_dec; simpl.
+      apply guardb_equiv in H. rewrite H.
+      assert (τ ∈ fun_step S σ (Some (Event x v))) by (apply fun_step_in; auto).
+      assert (τ ∈ equiv_on_list sensitivities σ).
+      { apply state_equiv_on_implies_list; auto. }
+      destruct (x ∈? space_input S); rewrite_in_list_dec; constructor; auto.
+
+  * intros σ e τ Hstep.
+    simpl in Hstep. unfold delay_space_step_fun in Hstep.
+    destruct e as [[x v] | ].
+    2:{ decompose_set_structure.
+        apply delay_space_internal.
+        { apply fun_in_step; auto. }
+        { rewrite rewrite_enumerate.
+          apply equiv_on_list_implies_state_equiv_on; auto.
+        }
+    }
+    destruct (x ∈? space_input S); rewrite_in_list_dec.
+    { decompose_set_structure.
+      apply delay_space_input; auto.
+      { apply fun_in_step; auto. }
+      { rewrite rewrite_enumerate.
+        apply equiv_on_list_implies_state_equiv_on; auto.
+      }
+    }
+    destruct (x ∈? space_output S); rewrite_in_list_dec.
+    { destruct (guardb σ) eqn:Hguard; [ simpl in Hstep | inversion Hstep].
+      decompose_set_structure.
+      apply delay_space_output; auto.
+      { apply guardb_equiv; auto. }
+      { apply fun_in_step; auto. }
+      { rewrite rewrite_enumerate.
+        apply equiv_on_list_implies_state_equiv_on; auto.
+      }
+    }
+    { simpl in Hstep. find_contradiction. }
+  Qed.
+
+End DelaySpace.
+
+Module Reflection := Structural_SS(name).
+Import Reflection.
+
+Section ISpace.
+
+  (* NO, this doesn't work because of the non-determinism introduced by Union/Eps transitions... *)
+
+  Notation "⊤" := (fun _ => True) : ensemble_notation.
+  Open Scope ensemble_notation.
+
+
+  Arguments enumerate {A} X {HX} : rename.
+
+
+  Fixpoint step_ISpace (S : ISpace) (σ : state name) (e : option (event name value))
+           : Ensemble (option (state name)) :=
+    match S with
+    | IFunc I0 x0 f0 => func_step_fun I0 x0 f0 σ e
+    | IUnion S1 S2 => 
+      match e with
+      | Some (Event x _) =>
+        if (in_list_dec x (ISpace_dom S1) && in_list_dec x (ISpace_dom S2))%bool
+        then step_ISpace S1 σ e ∩ step_ISpace S2 σ e
+        else if in_list_dec x (ISpace_dom S1)
+        then step_ISpace S1 σ e ∩ equiv_on_list (ISpace_dom S2) σ
+        else if in_list_dec x (ISpace_dom S2)
+        then step_ISpace S2 σ e ∩ equiv_on_list (ISpace_dom S1) σ
+        else ∅
+      | None =>
+        (step_ISpace S1 σ None ∩ equiv_on_list (ISpace_dom S2) σ)
+     ∪ (step_ISpace S2 σ None ∩ equiv_on_list (ISpace_dom S1) σ)
+      end
+
+    | IHide x0 S0 =>
+      match e with
+      | Some (Event y v) => if x0 =? y then ∅ else step_ISpace S0 σ e
+      | None => step_ISpace S0 σ None ∪ (fun τ => exists v, step_ISpace S0 σ (Some (Event x0 v)) τ)
+      end
+    | IFlop set reset clk old_clk D Q =>
+      flop_step_fun set reset clk old_clk D Q σ e
+    | IDelaySpace S0 sensitivities guard guardb =>
+      match e with
+      | Some (Event x _) =>
+        if in_list_dec x (ISpace_input S0)
+        then step_ISpace S0 σ e ∩ equiv_on_list sensitivities σ
+        else if (in_list_dec x (ISpace_output S) && guardb σ)%bool
+        then step_ISpace S0 σ e ∩ equiv_on_list sensitivities σ
+        else ∅
+      | None => step_ISpace S0 σ e ∩ equiv_on_list sensitivities σ
+      end
+    end.
+
+
+  Instance ISpace_functional : forall S, functional_step_relation (interp_ISpace S).
+  Proof.
+    induction S; simpl.
+    * apply func_functional.
+    * apply union_functional; auto; typeclasses eauto.
+    * apply hide_functional; auto; typeclasses eauto.
+    * apply flop_functional.
+    * apply delay_space_functional; auto.
+  Defined.
+
+  (*???*)
+  Instance ISpace_functional_correct : forall S `{ISpace_wf S},
+    functional_step_relation_correct (interp_ISpace S).
+  Proof.
+    induction S; intros wf; simpl.
+    * apply func_functional_correct.
+      inversion wf; auto.
+    * inversion wf; subst.
+      admit (*
+      apply union_functional_correct; auto. *).
+
+    * apply hide_functional_correct; auto. admit.
+      admit.
+    * apply flop_functional_correct. auto. admit.
+    * apply delay_space_functional_correct; auto.
+      admit.
+  Admitted.
+
+
+  Instance ISpace_enumerable : forall S,
+    enumerable (space_domain (interp_ISpace S)).
+  Proof.
+    intros.
+    apply functional_step_relation_enumerable_domain.
+    apply ISpace_functional.
+  Defined.
+
+
+  Lemma step_ISpace_correct : forall S σ e,
+    step_ISpace S σ e == fun_step (interp_ISpace S) σ e.
+  Proof.
+    induction S; intros σ e.
+    * simpl. reflexivity.
+    * simpl. unfold union_step_fun.
+      destruct e as [[x v] | ].
+      2:{ rewrite IHS1. rewrite IHS2.
+          rewrite (equiv_on_list_equiv (ISpace_dom S1)).
+          2:{ rewrite <- rewrite_enumerate.
+              rewrite <- space_domain_ISpace; reflexivity. 
+          }
+          rewrite (equiv_on_list_equiv (ISpace_dom S2)).
+(*                     (@enumerate _ (space_domain (interp_ISpace S2)) (ISpace_enumerable S2))).*)
+          2:{ rewrite <- rewrite_enumerate.
+              rewrite <- space_domain_ISpace; reflexivity. 
+          }
+          reflexivity.
+      }
+      rewrite <- (in_list_dec_equiv (ISpace_dom S1)
+                                  (enumerate (space_domain (interp_ISpace S1)))).
+      2:{ rewrite <- rewrite_enumerate.
+          rewrite <- space_domain_ISpace. reflexivity.
+      }
+      rewrite <- (in_list_dec_equiv (ISpace_dom S2)
+                                  (enumerate (space_domain (interp_ISpace S2)))).
+      2:{ rewrite <- rewrite_enumerate.
+          rewrite <- space_domain_ISpace. reflexivity.
+      }
+      destruct (in_list_dec x (ISpace_dom S1));
+      destruct (in_list_dec x (ISpace_dom S2));
+        simpl;
+      try rewrite IHS1; try rewrite IHS2; try reflexivity.
+      + rewrite (equiv_on_list_equiv (ISpace_dom S2)).
+          2:{ rewrite <- rewrite_enumerate.
+              rewrite <- space_domain_ISpace; reflexivity. 
+          }
+        reflexivity.
+      + rewrite (equiv_on_list_equiv (ISpace_dom S1)).
+          2:{ rewrite <- rewrite_enumerate.
+              rewrite <- space_domain_ISpace; reflexivity. 
+          }
+        reflexivity.
+    * simpl. unfold hide_step_fun.
+      destruct e as [[y v] | ].
+      { compare_next; auto. reflexivity. }
+      rewrite IHS.
+      apply union_mor; try reflexivity.
+      split; intros τ [v Hτ];
+        destruct (IHS σ (Some (Event x v))) as [IH1 IH2].
+      + exists v. apply IH1; auto.
+      + exists v. apply IH2; auto.
+
+    * simpl. reflexivity.
+
+    * simpl. unfold delay_space_step_fun.
+      destruct e as [[x v] | ].
+      2:{ rewrite IHS. reflexivity. }
+      rewrite <- (in_list_dec_equiv (ISpace_input S)
+                                  (enumerate (space_input (interp_ISpace S)))).
+      2:{ rewrite <- rewrite_enumerate.
+          rewrite <- space_input_ISpace. reflexivity.
+      }
+      rewrite <- (in_list_dec_equiv (ISpace_output S)
+                                  (enumerate (space_output (interp_ISpace S)))).
+      2:{ rewrite <- rewrite_enumerate.
+          rewrite <- space_output_ISpace. reflexivity.
+      }
+      destruct (in_list_dec x (ISpace_input S)) eqn:Hx.
+      { rewrite IHS. reflexivity. }
+      destruct (in_list_dec x (ISpace_output S)) eqn:Hx'; simpl.
+      2:{ reflexivity. }
+      destruct (guardb σ) eqn:Hguard.
+      { rewrite IHS. reflexivity. }
+      { reflexivity. }
+  Qed.
+
+
+
+  Theorem step_ISpace_in : forall S `{ISpace_wf S} σ e τ,
+    interp_ISpace S ⊢ σ →{e} τ ->
+    τ ∈ step_ISpace S σ e.
+  Proof.
+    intros.
+    rewrite step_ISpace_correct.
+    eapply fun_step_in; auto.
+  Unshelve. 
+    apply ISpace_functional_correct; auto.
+  Qed.
+  Theorem step_in_ISpace : forall S `{ISpace_wf S} σ e τ,
+    τ ∈ step_ISpace S σ e ->
+    interp_ISpace S ⊢ σ →{e} τ.
+  Proof.
+    intros S Hwf σ e τ Hτ.
+    set (H := @ISpace_functional_correct S Hwf).
+    rewrite step_ISpace_correct in Hτ.
+    eapply fun_in_step in Hτ; auto.
+  Qed.
+
+
+End ISpace.
+End FunctionalStateSpaces.
+
