StateSpace/MarkedGraphs.v
@@ -1,0 +1,286 @@
+Require Import Base.
+Require Import Circuit.
+Require Import Monad.
+Require Import Setoid.
+
+Require Import StateSpace.Definitions.
+Require Import StateSpace.Tactics.
+
+Require Import Program.Equality.
+
+Require Import List.
+Import ListNotations.
+Open Scope list_scope.
+
+Import EnsembleNotation.
+Open Scope ensemble_scope.
+
+Section MG_to_SS.
+
+  Set Implicit Arguments.
+  (** ** Convert a marked graph to a state space *)
+  Variable name : Set.
+  Context `{name_dec : eq_dec name}.
+
+  Variable transition : Set.
+  Context `{transition_dec : eq_dec transition}.
+  Variable MG : marked_graph transition.
+
+  Import EnsembleNotation.
+  Open Scope ensemble_scope.
+
+  Inductive place_eq : forall {t1 t2 t1' t2' : transition}, place MG t1 t2 -> place MG t1' t2' -> Prop :=
+  | place_refl : forall t1 t2 (p : place MG t1 t2), place_eq p p.
+
+
+  Class MG_naming_scheme :=
+  { transition_name : transition -> name
+  ; place_name : forall {t1 t2} (p : place MG t1 t2), name
+
+(*
+  ;  name_is_place_dec : forall (x : name),
+     {t1 : transition & {t2 : transition & {p : place MG t1 t2 & x = place_name p}}}
+   + {forall t1 t2 (p : place MG t1 t2), x <> place_name p}
+*)
+  ; name_to_place : name -> option {t1 & {t2 & place MG t1 t2}}
+  ; name_to_place_correct : forall x tin tout (p : place MG tin tout),
+        name_to_place x = Some (existT _ tin (existT _ tout p))
+    <-> x = place_name p
+
+  ; transition_update_value : transition -> value -> value
+
+  ; input_transition : Ensemble transition
+  ; input_transition_dec : `{in_dec input_transition}
+
+  ; transition_place_name_disjoint : forall t {t1 t2} (p : place MG t1 t2),
+    transition_name t <> place_name p
+
+    (* I'm not sure if t ∈ input_transition is the right restriction here, but
+    we need this fact for proving well_formed, and it does not hold without this
+    transition for click, e.g. with CLK+ and CLK-. On the other hand, what about
+    4 phase handshake protocols? *)
+  ; transition_name_injective : forall t t', t ∈ input_transition ->
+    t <> t' -> transition_name t <> transition_name t'
+
+   ; places_all_disjoint : forall {t1 t2 t1' t2' : transition}
+                                        (p : place MG t1 t2) (p' : place MG t1' t2'),
+      place_name p = place_name p' ->
+      place_eq p p'
+
+  }.
+  Context `{MG_scheme : MG_naming_scheme}.
+
+  Definition places_set : Ensemble name :=
+    fun x => exists t1 t2 (p : place MG t1 t2), x = place_name p.
+  Definition state_to_marking (σ : state name) : marking MG :=
+    fun t1 t2 p => val_to_nat (σ (place_name p)).
+
+  Lemma name_to_place_eq : forall t1 t2 (p : place MG t1 t2),
+    name_to_place (place_name p) = Some (existT _ t1 (existT _ t2 p)).
+  Proof.
+    intros.
+    apply name_to_place_correct; auto.
+  Qed.
+  Lemma name_to_place_neq : forall t,
+    name_to_place (transition_name t) = None.
+  Proof.
+    intros t.
+    destruct (name_to_place (transition_name t)) as [[t1 [t2 p]] | ] eqn:contra; auto.
+    apply name_to_place_correct in contra.
+    apply transition_place_name_disjoint in contra.
+    contradiction.
+  Qed.
+
+  Definition fire_in_state (t : transition) (σ : state name) : state name :=
+    fun x =>
+    match name_to_place x with
+    (* if x is not a place, do nothing *)
+    | None => σ x
+    | Some (existT _ tin (existT _ tout p)) =>
+         (* corner case: do nothing *)
+         if tin =? tout then σ x
+         (* if x is a place leading into t, increment the value *)
+         else if t =? tout then dec_value (σ x)
+         (* if x is a place leading out of t, decrement the value *)
+         else if t =? tin then inc_value (σ x)
+         (* otherwise do nothing *)
+         else σ x
+    end.
+
+  (* NOTE: this may not be the right relation for all marked graphs--get example from Peter *)
+  Let transition_set : Ensemble name := fmap transition_name (fun (t : transition) => True).
+
+  Inductive MG_SS_step
+    : state name -> option (event name value) -> option (state name) -> Prop :=
+
+  | transition_enabled σ σ' x v (t : transition) :
+    x = transition_name t ->
+    is_enabled MG t (state_to_marking σ) ->
+    v = transition_update_value t (σ x) ->
+    state_equiv_on (transition_set ∪ places_set)
+                   (Some σ') 
+                   (Some (update (fire_in_state t σ) x v)) ->
+    MG_SS_step σ (Some (Event x v)) (Some σ')
+
+  | input_not_enabled σ x v t :
+    x = transition_name t ->
+    t ∈ input_transition ->
+    ~ is_enabled MG t (state_to_marking σ) ->
+   MG_SS_step σ (Some (Event x v)) None
+  .
+
+  Let output_transition : Ensemble transition :=
+    (fun t => True) ∖ input_transition.
+(*    fun t => t ∉ input_transition.*)
+  Definition MG_SS : StateSpace name :=
+  {| space_input := fmap transition_name input_transition
+   ; space_output := fmap transition_name output_transition
+   ; space_internal := places_set
+   ; space_step := MG_SS_step
+   |}.
+
+  Lemma places_all_numbers_step : forall σ σ' e {t1 t2} (p : place MG t1 t2),
+    σ (place_name p) <> X ->
+    MG_SS ⊢ σ →{e} Some σ' ->
+    σ' (place_name p) <> X.
+  Proof.
+    intros σ σ' e t1 t2 p Hwf Hstep.
+    inversion Hstep; subst.
+    rewrite H5.
+    2:{ right. exists t1. exists t2. exists p. reflexivity. }
+    unfold update.
+    set (Hneq := transition_place_name_disjoint t p).
+    reduce_eqb.
+    unfold fire_in_state.
+    rewrite name_to_place_eq.
+    compare_next; auto.
+    compare_next; auto.
+    { destruct (σ (place_name p)); find_contradiction. }
+    compare_next; auto.
+    { destruct (σ (place_name p)); find_contradiction. }
+  Qed.
+
+
+  Lemma places_all_numbers : forall σ σ' tr {t1 t2} (p : place MG t1 t2),
+    σ (place_name p) <> X ->
+    MG_SS ⊢ σ →*{tr} Some σ' ->
+    σ' (place_name p) <> X.
+  Proof.
+    intros ? ? ? ? ? ? ? Hstep.
+    remember MG_SS as S.
+    remember (Some σ') as τ.
+    generalize dependent σ'.
+    generalize dependent t2. generalize dependent t1.
+    induction Hstep; intros t1 t2 p Hneq σ'' Hτ; subst.
+    * inversion Hτ; subst; auto.
+    * destruct e as [x v].
+      inversion H; subst; clear H.
+      rewrite H7.
+        2:{ right. do 3 eexists. reflexivity. }
+        unfold update.
+        set (Hneq' := transition_place_name_disjoint t0 p).
+        reduce_eqb.
+        unfold fire_in_state.
+        rewrite name_to_place_eq.
+        specialize (IHHstep _ _ p Hneq σ' eq_refl).
+        compare_next; auto.
+        compare_next; auto.
+        { destruct (σ' (place_name p)); find_contradiction. }
+        compare_next; auto.
+        { destruct (σ' (place_name p)); find_contradiction. }
+
+    * inversion H.
+  Qed.
+
+  Arguments well_formed {name}.
+  Lemma wf_MG_SS : well_formed MG_SS.
+  Proof.
+    set (Hdec := input_transition_dec).
+    constructor;
+    try match goal with
+    | [ |- _ ⊥ _ ] =>
+      simpl; constructor;
+      intros x Hx; deep_decompose_set_structure;
+      match goal with
+      | [ H : transition_name ?t1 = transition_name ?t2 |- _ ] =>
+        compare t1 t2;
+        try (eapply transition_name_injective; eauto; fail)
+
+      | [ H : transition_name ?t = place_name ?p |- _ ] =>
+        let Hdisjoint := fresh "Hdisjoint" in
+        set (Hdisjoint := transition_place_name_disjoint t p);
+        find_contradiction
+      end
+    end.
+
+    * intros ? ? ? ? Hstep.
+      inversion Hstep; subst; simpl.
+      { destruct (t ∈? input_transition).
+        + left. econstructor; eauto.
+        + right. econstructor; split; eauto.
+          unfold output_transition. solve_set.
+       }
+      { destruct (t ∈? input_transition).
+        + left. econstructor; eauto.
+        + right. econstructor; split; eauto.
+          unfold output_transition. solve_set.
+       }
+    * intros ? ? ? Hstep ? He Hexternal.
+      inversion Hstep; subst.
+      rewrite H5.
+      2:{ simpl in Hexternal. deep_decompose_set_structure; subst;
+          left; exists x0; split; auto; constructor.
+      }
+      unfold update.
+      compare_next; auto.
+      { contradiction (He (transition_update_value t (σ (transition_name t)))); auto. }
+      unfold fire_in_state.
+      assert (Hx : forall t1 t2 (p : place MG t1 t2), x <> place_name p).
+      { simpl in Hexternal. deep_decompose_set_structure; subst;
+        apply transition_place_name_disjoint.
+      }
+      assert (Hx' : name_to_place x = None).
+      { simpl in Hexternal; deep_decompose_set_structure; subst;
+          rewrite name_to_place_neq; auto.
+      }
+      rewrite Hx'; auto.
+
+    * intros ? ? ? ? Hstep.
+      inversion Hstep; subst.
+      rewrite H6.
+      2:{ left. exists t; split; auto; constructor. }
+      unfold update; simpl.
+      reduce_eqb. auto.
+  Qed.
+
+
+
+  Lemma MG_SS_val_not_X : forall σ0 tr σ,
+    MG_SS ⊢ σ0 →*{tr} Some σ ->
+    forall {t1 t2} (p : place MG t1 t2), 
+    σ0 (place_name p) <> X ->
+    σ (place_name p) <> X.
+  Proof.
+    intros σ0 tr σ Hstep.
+    remember (Some σ) as τ; generalize dependent σ.
+    induction Hstep; intros σ Hτ t1 t2 p Hwf; inversion Hτ; subst; auto.
+    * specialize (IHHstep σ' eq_refl t1 t2 p Hwf).
+      inversion H; subst.
+      rewrite H7.
+      2:{ right. eexists. eexists. exists p. reflexivity. }
+      unfold update. compare_next.
+      { apply transition_place_name_disjoint in Heq; contradiction.
+      }
+      unfold fire_in_state.
+      rewrite name_to_place_eq.
+      compare_next; auto.
+      compare_next. { destruct (σ' (place_name p)); try (inversion 1; fail); find_contradiction. }
+      compare_next. { destruct (σ' (place_name p)); try (inversion 1; fail); find_contradiction. }
+      auto.
+
+    * specialize (IHHstep σ' eq_refl t1 t2 p Hwf).
+      inversion H; subst.
+  Qed.
+
+  Unset Implicit Arguments.
+End MG_to_SS.
