StateSpace/Reflection.v
@@ -1,0 +1,338 @@
+Require Import Base.
+Require Import Circuit.
+Require Import Monad.
+Require Import Setoid.
+
+Require Import StateSpace.Definitions.
+Require Import StateSpace.Tactics.
+
+Require Import Program.Equality.
+
+Require Import List.
+Import ListNotations.
+Open Scope list_scope.
+
+Import EnsembleNotation.
+Open Scope ensemble_scope.
+
+
+
+
+Module Structural_SS (Export name : NameType).
+
+  Inductive ISpace :=
+  | IFunc (I : list name) (x : name) (f : state name -> value) : ISpace
+  | IUnion (S1 S2 : ISpace) : ISpace
+  | IHide  (x : name) (S : ISpace) : ISpace
+  | IFlop (set reset clk old_clk D Q : name) : 
+    (*all_disjoint [set;reset;clk;old_clk;D;Q] ->*)
+    ISpace
+  | IDelaySpace (S : ISpace)
+                (sensitivities : list name)
+                (guard : state name -> Prop)
+                (guardb : state name -> bool) : ISpace
+(*  | IPrim : StateSpace name -> ISpace*)
+  .
+
+  Fixpoint interp_ISpace (S : ISpace) : StateSpace name :=
+    match S with
+(*    | IPrim S0     => S0*)
+    | IFunc I' x f  => func_space I' x f
+    | IUnion S1 S2 => interp_ISpace S1 ∥ interp_ISpace S2
+    | IHide x S0   => hide x (interp_ISpace S0)
+    | IFlop set reset clk old_clk D Q => flop set reset clk old_clk D Q
+    | IDelaySpace S0 sens guard guardb => delay_space (interp_ISpace S0) sens guard guardb
+    end.
+
+  Fixpoint ISpace_dom (S : ISpace) : list name :=
+    match S with
+    | IFunc I0 x0 f0 => x0 :: I0
+    | IUnion S1 S2 => ISpace_dom S1 ++ ISpace_dom S2
+    | IHide x0 S0  => ISpace_dom S0
+    | IFlop set reset clk old_clk D Q => set::reset::clk::old_clk::D::Q::nil
+    | IDelaySpace S0 sens guard guardb => ISpace_dom S0 ++ sens
+    end.
+
+  Fixpoint ISpace_output (S : ISpace) : list name :=
+    match S with
+    | IFunc I0 x0 f0 => x0 :: nil
+    | IUnion S1 S2 => ISpace_output S1 ++ ISpace_output S2
+    | IHide x0 S0  => better_filter (fun y => negb (x0 =? y)) (ISpace_output S0)
+    | IFlop set reset clk old_clk D Q => Q::nil
+    | IDelaySpace S0 sens guard guardb => ISpace_output S0
+    end.
+
+  Fixpoint ISpace_input (S : ISpace) : list name :=
+    match S with
+    | IFunc I0 x0 f0 => I0
+    | IUnion S1 S2 => list_setminus (ISpace_input S1) (ISpace_output S2)
+                   ++ list_setminus (ISpace_input S2) (ISpace_output S1)
+    | IHide x0 S0  => ISpace_input S0
+    | IFlop set reset clk old_clk D Q => set::reset::clk::D::nil
+    | IDelaySpace S0 sens guard guardb => ISpace_input S0 ++ sens
+    end.
+
+  Fixpoint ISpace_internal (S : ISpace) : list name :=
+    match S with
+    | IFunc I0 x0 f0 => nil
+    | IUnion S1 S2 => ISpace_internal S1 ++ ISpace_internal S2
+    | IHide x0 S0  => x0 :: ISpace_internal S0
+    | IFlop set reset clk old_clk D Q => old_clk::nil
+    | IDelaySpace S0 sens guard guardb => ISpace_internal S0
+    end.
+
+  Lemma space_domain_ISpace : forall S,
+    space_domain (interp_ISpace S) == from_list (ISpace_dom S).
+  Proof.
+(*
+    induction S; unfold space_domain in *; simpl;
+      try rewrite from_list_app;
+      split; intros z Hz;
+      decompose_set_structure; try solve_set;
+      try rewrite <- IHS1 in *;
+      try rewrite <- IHS2 in *;
+      decompose_set_structure;
+      try solve_set.
+      try rewrite <- IHS1 in *.
+      rewrite <- IHS1 in H.
+      rewrite 
+*)
+  Admitted.
+
+  Lemma space_output_ISpace : forall S,
+    space_output (interp_ISpace S) == from_list (ISpace_output S).
+  Proof.
+  Admitted.
+
+  Lemma space_input_ISpace : forall S,
+    space_input (interp_ISpace S) == from_list (ISpace_input S).
+  Proof.
+  Admitted.
+  Lemma space_internal_ISpace : forall S,
+    space_internal (interp_ISpace S) == from_list (ISpace_internal S).
+  Proof.
+  Admitted.
+
+
+
+  Inductive ISpace_wf : ISpace -> Prop :=
+  | IFunc_wf : forall I x f,
+    x ∉ from_list I ->
+    ISpace_wf (IFunc I x f)
+  | IUnion_wf S1 S2 :
+    list_intersection (ISpace_internal S1) (ISpace_dom S2) = nil ->
+    list_intersection (ISpace_internal S2) (ISpace_dom S1) = nil ->
+    ISpace_wf S1 ->
+    ISpace_wf S2 ->
+    ISpace_wf (IUnion S1 S2)
+  (* more... *)
+  .
+  
+
+  Lemma interp_ISpace_wf : forall S,
+    ISpace_wf S ->
+    well_formed (interp_ISpace S).
+  Abort.
+
+
+  Ltac reflect_ISpace S :=
+  match S with
+  | func_space ?I0 ?x ?f => constr:(IFunc I0 x f)
+  | ?S1 ∥ ?S2            => let SS1 := reflect_ISpace S1 in
+                            let SS2 := reflect_ISpace S2 in
+                            constr:(IUnion SS1 SS2)
+  | hide ?x ?S'          => let SSS' := reflect_ISpace S' in
+                            constr:(IHide x SSS')
+  | flop ?set ?reset ?clk ?old_clk ?D ?Q => constr:(IFlop set reset clk old_clk D Q)
+  | delay_space ?S0 ?sens ?guard  ?guardb    => let SS := reflect_ISpace S0 in
+                                      constr:(IDelaySpace SS sens guard guardb)
+(*  | _                              => constr:(IPrim S)*)
+  end.
+  Ltac reflect_S S := 
+    let S' := reflect_ISpace S in
+    replace S with (interp_ISpace S') by reflexivity.
+  Module SSTactics := StateSpaceTactics(name).
+  Import SSTactics.
+
+  Ltac reflect_StateSpace :=
+  match goal with
+  | [ |- ?S1 = ?S2 ] => unfold_StateSpace S1;
+                        unfold_StateSpace S2;
+    match goal with
+    | [ |- ?S1' = ?S2' ] => reflect_S S1'; reflect_S S2'
+    end
+  end.
+
+  Section Test.
+  Variable x : name.
+  Let S : StateSpace name := C_elem x x x.
+  Let S' := (S ∥ func_space (x::nil) x (fun _ => X)).
+  Lemma foo : S' = S.
+    assert (Heq : S' = S') by reflexivity.
+    unfold_StateSpace S' in Heq.
+    reflect_StateSpace.
+  Abort.
+  End Test.
+
+
+  Definition update_oevent (σ : state name) (e : option (event name value)) : state name :=
+    match e with
+    | None => σ
+    | Some (Event x v) => update σ x v
+    end.
+
+
+
+ (* Set reflection, with ISpaces built in  *)
+
+  Inductive SetStructure :=
+  | SetEmpty : SetStructure
+  | SetSingleton : name -> SetStructure
+  | SetList : list name -> SetStructure
+  | SetUnion : SetStructure  -> SetStructure -> SetStructure
+  | SetIntersection : SetStructure -> SetStructure -> SetStructure
+  | SetDifference : SetStructure -> SetStructure -> SetStructure
+  | SetSpaceDomain : ISpace -> SetStructure
+  | SetSpaceInput : ISpace -> SetStructure
+  | SetSpaceOutput : ISpace -> SetStructure
+  | SetSpaceInternal : ISpace -> SetStructure
+  .
+
+  Ltac reflect_to_SetStructure S :=
+  match S with
+  | ∅ => constr:(SetEmpty)
+  | singleton ?x => constr:(SetSingleton x)
+  | ?S1 ∪ ?S2 => let l1 := reflect_to_SetStructure S1 in
+                  let l2 := reflect_to_SetStructure S2 in
+                  constr:(SetUnion l1 l2)
+  | space_domain ?S0 => let S0' := reflect_ISpace S0 in
+                        constr:(SetSpaceDomain S0')
+  | space_input ?S0 => let S0' := reflect_ISpace S0 in
+                        constr:(SetSpaceInput S0')
+  | space_output ?S0 => let S0' := reflect_ISpace S0 in
+                        constr:(SetSpaceOutput S0')
+  | space_internal ?S0 => let S0' := reflect_ISpace S0 in
+                        constr:(SetSpaceInternal S0')
+
+  | ?S1 ∖ ?S2 =>  let l1 := reflect_to_SetStructure S1 in
+                  let l2 := reflect_to_SetStructure S2 in
+                  constr:(SetDifference l1 l2)
+  | ?S1 ∩ ?S2 =>  let l1 := reflect_to_SetStructure S1 in
+                  let l2 := reflect_to_SetStructure S2 in
+                  constr:(SetIntersection l1 l2)
+  | from_list ?l0 => constr:(SetList l0)
+  end.
+
+  Fixpoint interpret_SetStructure S :=
+  match S with
+  | SetEmpty => ∅
+  | SetSingleton x => singleton x
+  | SetList l => from_list l
+  | SetUnion S1 S2 => interpret_SetStructure S1 ∪ interpret_SetStructure S2
+  | SetIntersection S1 S2 => (interpret_SetStructure S1)
+                           ∩ (interpret_SetStructure S2)
+  | SetDifference S1 S2 => (interpret_SetStructure S1)
+                         ∖ (interpret_SetStructure S2)
+  | SetSpaceDomain S0 => space_domain (interp_ISpace S0)
+  | SetSpaceInput S0 => space_input (interp_ISpace S0)
+  | SetSpaceOutput S0 => space_output (interp_ISpace S0)
+  | SetSpaceInternal S0 => space_internal (interp_ISpace S0)
+  end.
+
+  Fixpoint SetStructure_to_list S :=
+  match S with
+  | SetEmpty => nil
+  | SetSingleton x => x::nil
+  | SetList l => l
+  | SetUnion S1 S2 => SetStructure_to_list S1 ++ SetStructure_to_list S2
+  | SetIntersection S1 S2 => list_intersection (SetStructure_to_list S1)
+                                               (SetStructure_to_list S2)
+  | SetDifference S1 S2 => list_setminus  (SetStructure_to_list S1)
+                                          (SetStructure_to_list S2)
+  | SetSpaceDomain S0 => ISpace_dom S0
+  | SetSpaceInput S0 => ISpace_input S0
+  | SetSpaceOutput S0 => ISpace_output S0
+  | SetSpaceInternal S0 => ISpace_internal S0
+  end.
+
+  Lemma SetStructure_to_list_correct : forall S,
+    interpret_SetStructure S == from_list (SetStructure_to_list S).
+  Proof.
+  Admitted.
+
+  Ltac set_to_list HS S :=
+    let S0 := reflect_to_SetStructure S in
+    let l0 := eval simpl in (SetStructure_to_list S0) in
+    assert (HS : S == from_list l0);
+    [ transitivity (interpret_SetStructure S0);
+      [ reflexivity | rewrite SetStructure_to_list_correct; reflexivity]
+    | ].
+
+  (** * Solve goal of the form x ∈ S or x ∉ S by reflection. *)
+  Ltac solve_space_set :=
+  match goal with
+  | [ |- ?x ∈ ?S ] => let H := fresh "H" in
+                      set_to_list H S; rewrite H; clear H;
+                      to_in_list_dec; unfold in_list_dec; reduce_eqb; auto;
+                      simpl; reduce_eqb; auto
+  | [ |- ?x ∉ ?S ] => let H := fresh "H" in
+                      set_to_list H S; rewrite H; clear H;
+                      to_in_list_dec; unfold in_list_dec; reduce_eqb; auto;
+                      simpl; reduce_eqb; auto
+  end.
+
+
+  Ltac space_domain_to_list Hdom S :=
+  let l := fresh "l" in
+  evar (l : list name);
+  assert (Hdom : space_domain S == from_list l);
+  [ unfold_StateSpace S;
+    match goal with
+    | [ |- space_domain ?S == _ ] => let S' := reflect_ISpace S in
+                                     transitivity (space_domain (interp_ISpace S'));
+                                     [ reflexivity | ]
+    end;
+    rewrite space_domain_ISpace;
+    unfold l;
+    reflexivity
+  | simpl in l;
+    unfold l in Hdom;
+    clear l
+    ].
+
+
+  Ltac compare_next_in_list_dec :=
+  match goal with
+  | [ Hstep : ?S ⊢ _ →{Some (Event ?x _)} _
+    |- context[ in_list_dec ?x (enumerate (space_domain ?S) _) ] ]=>
+    let Hdom := fresh "Hdom" in
+    space_domain_to_list Hdom S;
+    rewrite Hdom;
+    rewrite <- rewrite_enumerate
+
+  | [ Hstep : ?S ⊢ _ →{Some (Event ?x _)} _
+    |- context[ in_list_dec ?x (enumerate (space_domain ?S) _) ] ]=>
+    let Hin := fresh "Hin" in
+    assert (Hin : x ∈ space_domain S)
+      by (apply wf_space in Hstep;
+           [unfold space_domain; solve_set | auto]);
+    rewrite rewrite_enumerate in Hin;
+    to_in_list_dec;
+    rewrite Hin;
+    clear Hin;
+    simpl
+  | [ Hevent : ~ event_in ?X (Some (Event ?x _))
+    |- context[ in_list_dec ?x (enumerate ?X _) ] ] =>
+    let Hin := fresh "Hin" in
+    assert (Hin : x ∉ X)
+      by (intro; contradict Hevent; constructor; auto);
+    rewrite rewrite_enumerate in Hin;
+    to_in_list_dec;
+    rewrite Hin;
+    clear Hin;
+    simpl
+  end.
+
+
+
+End Structural_SS.
