StateSpace/RelateTrace.v
@@ -1,0 +1,235 @@
+Require Import Base.
+Require Import Circuit.
+Require Import Monad.
+Require Import Setoid.
+
+Require Import StateSpace.Definitions.
+
+Require Import List.
+Import ListNotations.
+Open Scope list_scope.
+
+Import EnsembleNotation.
+Open Scope ensemble_scope.
+
+
+Section RelateTrace.
+
+  Context (name : Set) `{name_dec : eq_dec name}.
+
+  Variable S1 S2 : StateSpace name.
+  Variable σ1_0 σ2_0 : state name.
+  Hypothesis init_domain_consistent :
+    forall x, x ∈ space_domain S1 ->
+              x ∈ space_domain S2 ->
+              σ1_0 x = σ2_0 x.
+
+  (* input(SS1)=input(SS2)
+     output(SS1)=output(SS2) *)
+  Inductive relate_trace : state name -> trace name value -> state name -> Prop :=
+  | relate_trace_nil :
+    relate_trace σ1_0 t_empty σ2_0
+
+  | relate_trace_left σ1 σ1' σ2 t :
+    relate_trace σ1 t σ2 ->
+    S1 ⊢ σ1 →{None} Some σ1' ->
+    relate_trace σ1' t σ2
+
+  | relate_trace_right σ1 σ2 σ2' t :
+    relate_trace σ1 t σ2 ->
+    S2 ⊢ σ2 →{None} Some σ2' ->
+    relate_trace σ1 t σ2'
+
+  | relate_trace_sync σ1 σ1' σ2 σ2' t e :
+    relate_trace σ1 t σ2 ->
+    S1 ⊢ σ1 →{Some e} Some σ1' ->
+    S2 ⊢ σ2 →{Some e} Some σ2' ->
+    relate_trace σ1' (t ▶ e) σ2'.
+
+  Hypothesis internal_disjoint_1 : space_internal S1 ⊥ space_domain S2.
+  Hypothesis internal_disjoint_2 : space_internal S2 ⊥ space_domain S1.
+
+  Lemma relate_trace_domain : forall σ1 σ2 t,
+    well_formed S1 ->
+    well_formed S2 ->
+    relate_trace σ1 t σ2 ->
+    forall x, x ∈ space_domain S1 ->
+              x ∈ space_domain S2 ->
+              σ1 x = σ2 x.
+  Proof.
+    intros σ1 σ2 t Hwf1 Hwf2 Hrelate x Hx1 Hx2.
+    assert (x ∉ space_internal S1).
+    { (* if it were, it would be disjoint from dom(S2) *)
+      intro Hx.
+      find_contradiction.
+    }
+    assert (x ∉ space_internal S2).
+    { (* if it were, it would be disjoint from dom(S1) *)
+      intros Hx.
+      find_contradiction.
+    }
+
+    induction Hrelate.
+    * apply init_domain_consistent; auto.
+    * assert (Hσ1' : σ1' x = σ1 x).
+      { (* Since σ1 →{None} Some σ1', it must be the case that σ1 and σ1' only
+        differ on internal wires *)
+        eapply (wf_scoped _ Hwf1); eauto.
+        { intros v; inversion 1. }
+        { unfold space_domain in *. decompose_set_structure; solve_set. }
+      }
+      congruence.
+    * assert (Hσ2' : σ2' x = σ2 x).
+      { (* Since σ2 →{None} Some σ2', it must be the case that σ2 and σ2' only
+        differ on internal wires *)
+        eapply (wf_scoped _ Hwf2); eauto.
+        { intros v; inversion 1. }
+        { unfold space_domain in *. decompose_set_structure; solve_set. }
+      }
+      congruence.
+    * destruct e as [y v].
+      compare x y.
+      + (* x = y *)
+        assert (σ1' y = v).
+        { (* another feature of well-formed step relations *) 
+          eapply (wf_update _ Hwf1); eauto. 
+        }
+        assert (σ2' y = v).
+        { (* another feature of well-formed step relations *)
+          eapply (wf_update _ Hwf2); eauto.
+        }
+        congruence.
+      + (* x <> y *)
+        assert (σ1' x = σ1 x).
+        { (* σ1 and σ1' must only vary on interal wires and y *) 
+          eapply (wf_scoped _ Hwf1); eauto.
+          { intros v'; inversion 1; subst; find_contradiction. }
+          { unfold space_domain in *. decompose_set_structure; solve_set. }
+        }
+        assert (σ2' x = σ2 x).
+        { (* σ2 and σ2' must only vary on interal wires and y *)
+          eapply (wf_scoped _ Hwf2); eauto.
+          { intros v'; inversion 1; subst; find_contradiction. }
+          { unfold space_domain in *. decompose_set_structure; solve_set. }
+        }
+        congruence.
+  Qed.
+
+  Definition relate_trace_step_lemma := forall σ1 σ1' σ2 e t,
+    S1 ⊢ σ1 →{Some e} Some σ1' ->
+    relate_trace σ1 t σ2 ->
+    exists σ2', S2 ⊢ σ2 →{Some e} Some σ2'.
+
+
+  Theorem relate_trace_subset_lemma :
+    relate_trace_step_lemma ->
+    forall (σ1 : state name) t,
+      S1 ⊢ σ1_0 →*{t} Some σ1 ->
+      exists σ2, relate_trace σ1 t σ2.
+  Proof.
+    intros Hlemma σ1 t Hstep.
+    remember (Some σ1) as τ1 eqn:Heqτ.
+      generalize dependent σ1.
+    induction Hstep as [ | | ]; intros σ1 Heqτ; subst.
+    * inversion Heqτ; subst. rewrite <- H0.
+      exists σ2_0. constructor.
+    * unfold relate_trace_step_lemma in Hlemma.
+      rename σ' into σ1'.
+      destruct (IHHstep σ1' eq_refl) as [σ2' IH].
+      specialize (Hlemma _ _ _ _ _ H IH).
+      destruct Hlemma as [σ2 Hstep2].
+      exists σ2.
+      eapply relate_trace_sync; eauto.
+    * rename σ' into σ1'.
+      destruct (IHHstep σ1' eq_refl) as [σ2' IH].
+      exists σ2'.
+      eapply relate_trace_left; eauto.
+  Qed.
+
+  Lemma relate_trace_project_left : forall σ1 t σ2,
+      relate_trace σ1 t σ2 ->
+      S1 ⊢ σ1_0 →*{t} Some σ1.
+  Proof.
+    intros σ1 t σ2 Hrelate.
+    induction Hrelate.
+    * constructor.
+    * eapply stepsEps; eauto.
+    * apply IHHrelate.
+    * eapply steps1; eauto.
+  Qed.
+
+  Lemma relate_trace_project_right : forall σ1 t σ2,
+      relate_trace σ1 t σ2 ->
+      S2 ⊢ σ2_0 →*{t} Some σ2.
+  Proof.
+    intros σ1 t σ2 Hrelate.
+    induction Hrelate.
+    * constructor.
+    * apply IHHrelate.
+    * eapply stepsEps; eauto.
+    * eapply steps1; eauto.
+  Qed.
+
+
+  Theorem relate_trace_step_subset :
+    relate_trace_step_lemma ->
+    traces_of S1 σ1_0 ⊆ traces_of S2 σ2_0.
+  Proof.
+    intros Hlemma t H1.
+    destruct H1 as [σ1 H1].
+    destruct (relate_trace_subset_lemma Hlemma _ _ H1) as [σ2 Hrelate].
+    exists σ2.
+    eapply relate_trace_project_right; eauto.
+  Qed.
+
+End RelateTrace.
+
+
+Section UnionStateSpaceRefinement.
+
+  Context {name : Set} `{name_dec : eq_dec name}.
+  Variable S1 S2 S1' S2' : StateSpace name.
+  Variable σ0 σ0' : state name.
+
+  Theorem union_refinement : 
+    state_equiv_on (space_domain (S1 ∥ S2) ∩ space_domain (S1' ∥ S2'))
+                   (Some σ0) (Some σ0') ->
+    traces_of S1 σ0 ⊆ traces_of S1' σ0' ->
+    traces_of S2 σ0 ⊆ traces_of S2' σ0' ->
+    traces_of (S1 ∥ S2) σ0 ⊆ traces_of (S1' ∥ S2') σ0'.
+  Proof.
+    intros Hequiv H1 H2.
+    apply relate_trace_step_subset.
+    { intros x Hx Hx'.
+      apply Hequiv.
+      solve_set.
+    }
+    unfold relate_trace_step_lemma.
+    intros σ σ' σT e t Hstep1 Hrelate.
+
+    inversion Hrelate; subst.
+    * inversion Hstep1; subst.
+      + (* e ∉ domain S2 *)
+        assert (H1' : t_empty ▶ e ∈ traces_of S1' σT).
+        { apply H1.
+          exists σ'. econstructor; eauto. constructor.
+        }
+        destruct H1' as [σT' H1'].
+        assert (Hstep' : exists σT'', S1' ⊢ σT →{Some e} Some σT'') by admit (* lemma *).
+        destruct Hstep' as [σT'' Hstep'].
+        exists σT''.
+        Print union_step.
+        apply union_step_1; auto.
+        (* These  two rely on the relation between the domain of Si and the domain of Si'. *)
+        admit (* why? *).
+        admit (* why? *).
+      + (* e ∉ domain S1 *)
+        admit (* same as above *).
+      + admit.
+
+  Abort.
+
+
+      
+End UnionStateSpaceRefinement.
+
