StateSpace/Tactics.v
@@ -1,0 +1,399 @@
+Require Import Base.
+Require Import Circuit.
+Require Import Monad.
+Require Import Setoid.
+
+Require Import StateSpace.Definitions.
+
+Require Import List.
+Import ListNotations.
+Open Scope list_scope.
+
+Import EnsembleNotation.
+Open Scope ensemble_scope.
+
+Module Type NameType.
+  Parameter name : Set.
+  Parameter name_eq_dec : eq_dec name.
+  Existing Instance name_eq_dec.
+  Export EnsembleNotation.
+  Open Scope ensemble_scope.
+
+End NameType.
+
+Module StateSpaceTactics (Export name : NameType).
+
+  Add Parametric Morphism : event_in
+    with signature Same_set name ==> @eq (option (event name value)) ==> iff as event_in_equiv.
+  Proof.
+    intros.
+    apply event_in_equiv; auto.
+  Qed.
+  Add Parametric Morphism : state_equiv_on
+    with signature (Same_set name) ==> (@eq (option (state name)))
+                                   ==> (@eq (option (state name))) ==> iff
+    as state_equiv_on_equiv.
+  Proof.
+    intros.
+    apply state_equiv_on_equiv; auto.
+  Qed.
+
+  Ltac rewrite_state_equiv :=
+  match goal with
+  | [ H : state_equiv_on ?X (Some ?σ') (Some _) |- context[?σ' _] ] =>
+    rewrite H; [ try unfold update | decompose_set_structure]
+  | [ H : state_equiv_on ?X (Some _) (Some ?σ') |- context[?σ' _] ] =>
+    rewrite <- H; [ try unfold update | decompose_set_structure]
+  end.
+
+
+  Ltac rewrite_state_equiv_branch y :=
+  match goal with
+  | [ Hequiv : state_equiv_on ?X (Some ?σ) (Some ?σ')
+    |- context[ ?σ' y ] ] =>
+      let Hy := fresh "Hy" in
+      destruct (y ∈? X) as [Hy | Hy];
+        [ rewrite_state_equiv | clear Hequiv]
+  end.
+
+
+  Lemma union_inversion_left : forall (S1 S2 : StateSpace name) σ x v σ',
+    (S1 ∥ S2) ⊢ σ →{Some (Event x v)} Some σ' ->
+    x ∈ space_domain S1 ->
+    S1 ⊢ σ →{Some (Event x v)} Some σ'.
+  Proof.
+    intros ? ? ? ? ? ? Hstep Hdom.
+    inversion Hstep; subst; auto.
+    (* the only remaining case is when x ∉ dom(S1), a contradiction *)
+    { absurd (event_in (space_domain S1) (Some (Event x v))); auto.
+      constructor; auto.
+    }
+  Qed.
+
+  Lemma union_inversion_left_only : forall (S1 S2 : StateSpace name) σ e σ',
+    (S1 ∥ S2) ⊢ σ →{e} Some σ' ->
+    event_in (space_domain S1) e ->
+    ~ event_in (space_domain S2) e ->
+    S1 ⊢ σ →{e} Some σ'
+    /\ state_equiv_on (space_domain S2) (Some σ) (Some σ').
+  Proof.
+    intros ? ? ? ? ? Hstep H1 H2.
+    inversion Hstep; subst; split; auto; 
+      try contradiction.
+    contradict H2.
+    inversion H; subst; auto;
+    match goal with
+    [ H : event_in (_ ?S2) ?e |- event_in (space_domain ?S2) ?e ] =>
+      inversion H; subst;
+      constructor;
+      unfold space_domain; solve_set
+    end.
+  Qed.
+
+  Lemma union_inversion_right : forall (S1 S2 : StateSpace name) σ x v σ',
+      (S1 ∥ S2) ⊢ σ →{Some (Event x v)} Some σ' ->
+      x ∈ space_domain S2 ->
+      S2 ⊢ σ →{Some (Event x v)} Some σ'.
+  Proof.
+    intros ? ? ? ? ? ? Hstep Hdom.
+    inversion Hstep; subst; auto.
+    (* the only remaining case is when x ∉ dom(S2), a contradiction *)
+    { absurd (event_in (space_domain S2) (Some (Event x v))); auto.
+      constructor; auto.
+    }
+  Qed.
+
+  Lemma union_inversion_right_only : forall (S1 S2 : StateSpace name) σ e σ',
+    (S1 ∥ S2) ⊢ σ →{e} Some σ' ->
+    ~ event_in (space_domain S1) e ->
+    event_in (space_domain S2) e ->
+    S2 ⊢ σ →{e} Some σ'
+    /\ state_equiv_on (space_domain S1) (Some σ) (Some σ').
+  Proof.
+    intros ? ? ? ? ? Hstep H1 H2.
+    inversion Hstep; subst; split; auto; 
+      try contradiction.
+    contradict H1.
+    inversion H; subst; auto;
+    match goal with
+    [ H : event_in (_ ?S2) ?e |- event_in (space_domain ?S2) ?e ] =>
+      inversion H; subst;
+      constructor;
+      unfold space_domain; solve_set
+    end.
+  Qed.
+
+  Lemma union_inversion_lr : forall (S1 S2 : StateSpace name) σ x v σ',
+    (S1 ∥ S2) ⊢ σ →{Some (Event x v)} Some σ' ->
+    x ∈ space_domain S1 ∩ space_domain S2 ->
+    S1 ⊢ σ →{Some (Event x v)} Some σ' /\ S2 ⊢ σ →{Some (Event x v)} Some σ'.
+  Proof.
+    intros ? ? ? ? ? ? Hstep Hdom.
+    split; [eapply union_inversion_left | eapply union_inversion_right];
+      eauto; decompose_set_structure.
+  Qed.
+
+  Lemma union_inversion : forall (S1 S2 : StateSpace name) e σ σ',
+    (S1 ∥ S2) ⊢ σ →{e} Some σ' ->
+    S1 ⊢ σ →{e} Some σ' \/ S2 ⊢ σ →{e} Some σ'.
+  Proof.
+    intros S1 S2 e σ σ' Hstep.
+    inversion Hstep; auto.
+  Qed.
+
+  Lemma union_inversion_None : forall (S1 S2 : StateSpace name) σ σ',
+    (S1 ∥ S2) ⊢ σ →{None} Some σ' ->
+       (S1 ⊢ σ →{None} Some σ' /\ state_equiv_on (space_domain S2) (Some σ) (Some σ'))
+    \/ (S2 ⊢ σ →{None} Some σ' /\ state_equiv_on (space_domain S1) (Some σ) (Some σ')).
+  Proof.
+    intros S1 S2 σ σ' Hstep.
+    inversion Hstep; subst; auto.
+    inversion H;
+    match goal with
+    | [ H : event_in _ None |- _ ] => inversion H
+    end.
+  Qed.
+
+
+(*
+  Instance internal_in_dec : forall l, in_dec (space_internal (latch_stage_with_env l)).
+  Proof.
+    intros l. simpl. typeclasses eauto.
+  Qed.
+
+  Instance input_in_dec : forall l, in_dec (space_input (latch_stage_with_env l)).
+  Admitted.
+
+  Instance output_in_dec : forall l, in_dec (space_output (latch_stage_with_env l)).
+  Admitted.
+*)
+
+
+  Lemma union_internal_inversion_right : forall (S1 S2 : StateSpace name) σ x v σ',
+      well_formed S1 ->
+      well_formed S2 ->
+      space_internal S1 ⊥ space_domain S2 ->
+      space_domain S1 ⊥ space_internal S2 ->
+      (S1 ∥ S2) ⊢ σ →{ Some (Event x v)} Some σ' ->
+      x ∉ space_domain S2 ->
+      state_equiv_on (space_internal S2) (Some σ') (Some σ).
+  Proof.
+    intros ? ? ? ? ? ? Hwf1 Hwf2 Hdisj1 Hdisj2 Hstep Hx y Hy.
+    inversion Hstep as [ ? ? H_event_in Hstep' Hequiv
+                       | ? ? H_event_in Hstep' Hequiv
+                       | ? ? Hevent Hstep1 Hstep2]; subst; auto.
+    * unfold state_equiv_on in Hequiv.
+      rewrite Hequiv; auto.
+      unfold space_domain; solve_set.
+    * contradict H_event_in.
+      constructor.
+      apply wf_space in Hstep; auto.
+      2:{ apply wf_union; auto. }
+      simpl in Hstep.
+      decompose_set_structure; unfold space_domain in *;
+        try solve_set;
+        try (contradict Hx; solve_set).
+
+    * inversion Hevent as [Hevent1 Hevent2 | Hevent1 Hevent2 | Hevent1 Hevent2];
+        inversion Hevent2; subst;
+          contradict Hx; unfold space_domain; solve_set.
+  Qed.
+
+  Lemma hide_inversion : forall (S : StateSpace name) σ x e σ',
+      (hide x S) ⊢ σ →{Some e} Some σ' ->
+      S ⊢ σ →{Some e} Some σ'.
+  Proof.
+    intros ? ? ? ? ? Hstep.
+    inversion Hstep; auto.
+  Qed.
+
+  Lemma hide_inversion_None : forall (S : StateSpace name) σ x σ',
+      (hide x S) ⊢ σ →{None} Some σ' ->
+      S ⊢ σ →{None} Some σ' \/ exists v, S ⊢ σ →{Some (Event x v)} Some σ'.
+  Proof.
+    intros ? ? ? ? Hstep.
+    inversion Hstep; subst; auto.
+    right. exists v. auto.
+  Qed.
+
+  Lemma func_space_output_inversion : forall I (o : name) f (σ : state name) x v σ',
+      o ∉ from_list I ->
+      func_space I o f ⊢ σ →{Some (Event x v)} Some σ' ->
+      x = o ->
+      v = f σ.
+  Proof.
+    intros ? ? ? ? ? ? ? Ho Hstep ?. subst.
+    inversion Hstep; try find_contradiction.
+    subst. auto.
+  Qed.
+
+
+  Lemma func_space_output_unstable : forall I (o : name) f σ x v σ',
+      o ∉ from_list I ->
+      func_space I o f ⊢ σ →{Some (Event x v)} Some σ' ->
+      x = o ->
+      σ x <> v.
+  Proof.
+    intros ? ? ? ? ? ? ? ? Hstep Heq.
+    subst.
+    inversion Hstep; subst; try find_contradiction; auto.
+  Qed.
+
+  Lemma func_space_output_neq : forall I (o : name) f σ v σ' y,
+      o ∉ from_list I ->
+      func_space I o f ⊢ σ →{Some (Event o v)} Some σ' ->
+      y ∈ from_list I ->
+      σ' y = σ y.
+  Proof.
+    intros ? ? ? ? ? ? ? ? Hstep Hneq.
+(*
+    inversion Hstep; subst;
+    match goal with
+    | [ H : state_equiv_on _ (Some ?σ') _ |- ?σ' _ = _ ] => rewrite H; [unfold update | try solve_set]
+    end;
+      compare_next; auto.
+  Qed.
+*)
+  Admitted.
+
+  Lemma func_space_inversion_None : forall I (o : name) f (σ : state name) σ',
+      func_space I o f ⊢ σ →{None} Some σ' ->
+      False.
+  Proof.
+    intros. inversion H.
+  Qed.
+
+Lemma func_space_inversion : forall I o f σ e σ',
+  o ∉ from_list I ->
+  func_space I o f ⊢ σ →{e} Some σ' ->
+  match e with
+  | None => False
+  | Some (Event y v) => state_equiv_on (from_list I ∪ singleton o) (Some (update σ y v)) (Some σ')
+                    /\ (y = o -> (v = f σ /\ f σ <> σ o))
+  end.
+Proof.
+  intros ? ? ? ? ? ? Hwf Hstep.
+  inversion Hstep; subst.
+  * split; auto.
+    intro Hi; subst; find_contradiction.
+  * split; auto.
+    intros Heq; subst; find_contradiction.
+  * split; auto.
+Qed.
+
+  Lemma flop_inversion_output : forall set reset clk old_clk D Q σ v σ',
+    all_disjoint [set; reset;clk;old_clk;D;Q] ->
+    σ set = Bit1 ->
+    σ reset = Bit1 ->
+    flop set reset clk old_clk D Q ⊢ σ →{Some (Event Q v)} Some σ' ->
+    σ clk = Bit1 /\
+    σ old_clk <> Bit1 /\
+    v = σ D /\
+     state_equiv_on (from_list [set;reset;clk;D;Q;old_clk])
+        (Some (update (update σ Q v) old_clk (σ clk)))
+        (Some σ').
+  Proof.
+    intros ? ? ? ? ? ? ? ? ? ? Hset Hreset Hstep.
+    inversion Hstep; subst; auto; clear Hstep.
+    + contradict H4. simpl. solve_set.
+    + find_contradiction.
+    + find_contradiction.
+  Qed.
+
+Ltac unfold_SS recurse_flag loc_flag S :=
+  match S with
+
+  | func_space ?I0 ?x ?f => idtac
+  | ?S1 ∥ ?S2            =>
+    (* If the recurse_flag is true then we want to unfold recursively; if false,
+    only unfold the head term, in this case, already a Union *)
+    maybe_do recurse_flag ltac:(unfold_SS recurse_flag loc_flag S1);
+    maybe_do recurse_flag ltac:(unfold_SS recurse_flag loc_flag S2)
+  | hide ?x ?S'          =>
+    maybe_do recurse_flag ltac:(unfold_SS recurse_flag loc_flag S')
+  | flop ?set ?reset ?clk ?old_clk ?D ?Q => idtac
+  | delay_space ?S0 ?sens ?guard ?guardb    => 
+    maybe_do recurse_flag ltac:(unfold_SS recurse_flag loc_flag S0)
+
+  (* func *)
+  | _ => let I := fresh "I" in
+         let o := fresh "o" in
+         let f := fresh "f" in
+         evar (I : list name);
+         evar (o : name);
+         evar (f : state name -> value);
+         replace_with_in S (func_space I o f) loc_flag;
+         unfold I, o, f in *;
+         clear I o f;
+         [ | reflexivity]
+                
+  (* union *)
+  | _ => let S1 := fresh "S1" in
+         let S2 := fresh "S2" in
+         evar (S1 : StateSpace name);
+         evar (S2 : StateSpace name);
+         replace_with_in S (S1 ∥ S2) loc_flag;
+         unfold S1, S2 in *;
+         [ | reflexivity];
+         maybe_do recurse_flag ltac:(let S1' := eval unfold S1 in S1 in
+                                let S2' := eval unfold S2 in S2 in
+                                unfold_SS recurse_flag loc_flag S1';
+                                unfold_SS recurse_flag loc_flag S2');
+         clear S1 S2
+  (* hide *)
+  | _ => let x0 := fresh "x0" in
+         let S0 := fresh "S0" in
+         evar (x0 : name);
+         evar (S0 : StateSpace name);
+         replace_with_in S (hide x0 S0) loc_flag;
+         unfold x0, S0 in *;
+         [ | reflexivity];
+         maybe_do recurse_flag ltac:(let S0' := eval unfold S0 in S0 in
+                                unfold_SS recurse_flag loc_flag S0');
+         clear x0 S0
+
+  (* flop *)
+  | _ => let set := fresh "set" in
+         let reset := fresh "reset" in
+         let clk := fresh "clk" in
+         let old_clk := fresh "old_clk" in
+         let D := fresh "D" in
+         let Q := fresh "Q" in
+         evar (set : name); evar (reset : name);
+         evar (clk : name); evar (old_clk : name);
+         evar (D : name); evar (Q : name);
+         replace_with_in S (flop set reset clk old_clk D Q) loc_flag;
+         unfold set, reset, clk, old_clk, D, Q in *;
+         clear set reset clk old_clk D Q;
+         [ | reflexivity]
+
+  (* delay space *)
+  | _ => let S0 := fresh "S0" in
+         let sens := fresh "sens" in
+         let guard := fresh "guard" in
+         let guardb := fresh "guardb" in
+         evar (S0 : StateSpace name);
+         evar (sens : list name);
+         evar (guard : state name -> Prop);
+         evar (guardb : state name -> bool);
+         replace_with_in S (delay_space S0 sens guard guardb) loc_flag;
+         unfold S0, sens, guard, guardb in *;
+         [ | reflexivity];
+         maybe_do recurse_flag ltac:(let S0' := eval unfold S0 in S0 in
+                                unfold_SS recurse_flag loc_flag S0');
+         clear S0 sens guard guardb
+  end.
+  Tactic Notation "unfold_StateSpace" constr(S) :=
+    (unfold_SS true false S).
+  Tactic Notation "unfold_StateSpace_1" constr(S) :=
+    (unfold_SS false false S).
+  Tactic Notation "unfold_StateSpace" constr(S) "in" "*" :=
+    (unfold_SS true true S).
+  Tactic Notation "unfold_StateSpace_1" constr(S) "in" "*" :=
+    (unfold_SS false true S).
+  Tactic Notation "unfold_StateSpace" constr(S) "in" hyp(H) :=
+    (unfold_SS true H S).
+  Tactic Notation "unfold_StateSpace_1" constr(S) "in" hyp(H) :=
+    (unfold_SS false H S).
+
+End StateSpaceTactics.
